Proof of RTac.Minify

theories/RTac/Minify.v
@@ -12,9 +12,12 @@ Require Import MirrorCore.RTac.Reduce.
 Require Import MirrorCore.Util.Forwardy.
 Require Import MirrorCore.Util.Nat.
 
-
 Set Implicit Arguments.
 Set Strict Implicit.
+
+(** TODO(gmalecha): This should be somewhere **)
+Instance Reflexive_ge : Reflexive ge.
+Proof. constructor. Qed.
 
 Section parameterized.
   Variable typ : Type.
@@ -54,6 +57,15 @@ Section parameterized.
       | Some u' => Some (lookup_compress es base u')
     end.
 
+  Fixpoint types_after_instantiate (ts : tenv typ) (inst : list (option expr))
+  : tenv typ :=
+    match ts , inst with
+      | nil , nil => nil
+      | t :: ts , None :: is => t :: types_after_instantiate ts is
+      | t :: ts , Some _ :: is => types_after_instantiate ts is
+      | _ , _ => nil
+    end.
+
   Section minify.
     Variable base : nat.
     Variables (c : Ctx typ expr) (cs : ctx_subst c).
@@ -71,12 +83,7 @@ Section parameterized.
               List.map (Functor.fmap
                           (instantiate (do_instantiate cs base (es ++ mlist))
                                        0)) mlist in
-          let tes := combine ts mlist_inst in
-          let tes' := filter (fun x => match snd x with
-                                         | None => true
-                                         | Some _ => false
-                                       end) tes in
-          let ts' := map fst tes' in
+          let ts' := types_after_instantiate ts mlist_inst in
           GExs_nil_check ts' (amap_empty _)
                          (minify_goal (es ++ mlist_inst) (len_ts + nus) g')
         | GHyp e g' =>
@@ -119,62 +126,170 @@ Section parameterized.
       do 2 constructor.
     Qed.
 
-    (** TODO: I can not capture the meaning of the terms in the list without
-     ** their corresponding environments
+    (** NOTE: You must have the environments to capture the meaning of
+     ** the terms semantically
      **)
 
-    Inductive mapD (_tus _tus' _tvs : tenv typ)
-    : forall tus tus' (es : list (option expr)),
+    Inductive mapD (_tus _tus' _tus_post' _tvs : tenv typ)
+    : forall (tus tus' : tenv typ) (es : list (option expr)),
+        (hlist typD _tus -> hlist typD _tus' -> hlist typD _tvs ->
+         hlist typD tus -> hlist typD tus' -> hlist typD _tus_post' -> Prop) -> Prop :=
+    | MD_nil : @mapD _tus _tus' _tus_post' _tvs nil nil nil (fun _ _ _ a b _ => a = b)
+    | MD_None : forall es t tus tus' P,
+        @mapD (_tus ++ t :: nil) (_tus' ++ t :: nil) _tus_post' _tvs tus tus' es P ->
+        @mapD _tus _tus' _tus_post' _tvs (t :: tus) (t :: tus') (None :: es)
+              (fun U U' V a b Upost =>
+                    hlist_hd a = hlist_hd b
+                 /\ P (hlist_app U (Hcons (hlist_hd a) Hnil))
+                      (hlist_app U' (Hcons (hlist_hd a) Hnil)) V
+                      (hlist_tl a) (hlist_tl b) Upost)
+    | MD_Some : forall e es t tus tus' P eD,
+        @mapD (_tus ++ t :: nil) _tus' _tus_post' _tvs tus tus' es P ->
+        exprD' (_tus' ++ tus' ++ _tus_post') _tvs e t = Some eD ->
+        @mapD _tus _tus' _tus_post' _tvs (t :: tus) tus' (Some e :: es)
+              (fun U U' V a b Upost =>
+                    hlist_hd a = eD (hlist_app U' (hlist_app b Upost)) V
+                 /\ P (hlist_app U (Hcons (hlist_hd a) Hnil))
+                      U' V (hlist_tl a) b Upost).
+
+    Arguments mapD {_ _ _ _} _ _ _ _.
+
+    Inductive mapD_nil (_tus _tus' _tvs : tenv typ)
+    : forall (tus tus' : tenv typ) (es : list (option expr)),
         (hlist typD _tus -> hlist typD _tus' -> hlist typD _tvs ->
          hlist typD tus -> hlist typD tus' -> Prop) -> Prop :=
-    | MD_nil : forall tus, @mapD _tus _tus' _tvs tus tus nil (fun _ _ _ a b => a = b)
-    | MD_None : forall es t tus tus' P,
-        @mapD (_tus ++ t :: nil) (_tus' ++ t :: nil) _tvs tus tus' es P ->
-        @mapD _tus _tus' _tvs (t :: tus) (t :: tus') (None :: es)
+    | MD_nil_nil : @mapD_nil _tus _tus' _tvs nil nil nil (fun _ _ _ a b => a = b)
+    | MD_nil_None : forall es t tus tus' P,
+        @mapD_nil (_tus ++ t :: nil) (_tus' ++ t :: nil) _tvs tus tus' es P ->
+        @mapD_nil _tus _tus' _tvs (t :: tus) (t :: tus') (None :: es)
               (fun U U' V a b =>
                     hlist_hd a = hlist_hd b
                  /\ P (hlist_app U (Hcons (hlist_hd a) Hnil))
                       (hlist_app U' (Hcons (hlist_hd a) Hnil)) V
                       (hlist_tl a) (hlist_tl b))
-    | MD_Some : forall e es t tus tus' P eD,
-        @mapD (_tus ++ t :: nil) _tus' _tvs tus tus' es P ->
+    | MD_nil_Some : forall e es t tus tus' P eD,
+        @mapD_nil (_tus ++ t :: nil) _tus' _tvs tus tus' es P ->
         exprD' (_tus' ++ tus') _tvs e t = Some eD ->
-        @mapD _tus _tus' _tvs (t :: tus) tus' (Some e :: es)
+        @mapD_nil _tus _tus' _tvs (t :: tus) tus' (Some e :: es)
               (fun U U' V a b =>
                     hlist_hd a = eD (hlist_app U' b) V
                  /\ P (hlist_app U (Hcons (hlist_hd a) Hnil))
                       U' V (hlist_tl a) b).
+    Arguments mapD_nil {_ _ _} _ _ _ _.
 
-    Arguments mapD {_ _ _} _ _ _ _.
-
-    (** TODO(gmalecha): move **)
-    Lemma nth_error_get_hlist_nth_conv
-      : forall T F ls ls' n (pf : ls' = ls),
-        @nth_error_get_hlist_nth T F ls n =
-        match pf in _ = ls'
-              return option { t : T & hlist F ls' -> F t }
-        with
-          | eq_refl => @nth_error_get_hlist_nth T F ls' n
-        end.
+    Theorem mapD_mapD_nil
+    : forall _tus _tus' _tvs tus tus' es R,
+        @mapD _tus _tus' nil _tvs tus tus' es R ->
+        exists R',
+          @mapD_nil _tus _tus' _tvs tus tus' es R' /\
+          forall _us _us' vs us us' us'',
+            R _us _us' vs us us' us'' ->
+            R' _us _us' vs us us'.
     Proof.
-      destruct pf; reflexivity.
+      remember (@nil typ). intros. revert Heql. induction H.
+      { eexists; split.
+        + constructor.
+        + simpl. auto. }
+      { intros. specialize (IHmapD Heql).
+        forward_reason.
+        eexists; split.
+        + constructor. eassumption.
+        + simpl. intros.
+          forward_reason; split; eauto. }
+      { intros. specialize (IHmapD Heql).
+        subst.
+        forward_reason.
+        rewrite exprD'_conv
+          with (pfv:=eq_refl) (pfu:=eq_sym (f_equal _ (app_nil_r_trans _)))
+            in H0.
+        autorewrite with eq_rw in H0. forwardy; inv_all; subst.
+        eexists; split.
+        + constructor. eassumption. eassumption.
+        + simpl. intros.
+          forward_reason; split; eauto.
+          rewrite H3; clear H3.
+          rewrite (hlist_eta us'').
+          rewrite hlist_app_nil_r.
+          clear.
+          generalize (app_nil_r_trans tus').
+          generalize (tus' ++ nil).
+          intros; subst. reflexivity. }
     Qed.
-    (** TODO(gmalecha): move to ExtLib.Data.SigT **)
-    Lemma eq_sigT_rw
-      : forall T U F (a b : T) (pf : a = b) s,
-        match pf in _ = x return @sigT U (F x) with
-          | eq_refl => s
-        end =
-        @existT U (F b) (projT1 s)
-                match pf in _ = x return F x (projT1 s) with
-                  | eq_refl => (projT2 s)
-                end.
-    Proof. destruct pf. destruct s; reflexivity. Qed.
 
-    Hint Rewrite eq_sigT_rw : eq_rw.
+    Theorem mapD_nil_mapD
+    : forall _tus _tus' _tvs tus tus' es R,
+        @mapD_nil _tus _tus' _tvs tus tus' es R ->
+        exists R',
+          @mapD _tus _tus' nil _tvs tus tus' es R' /\
+          forall _us _us' vs us us',
+            R _us _us' vs us us' ->
+            R' _us _us' vs us us' Hnil.
+    Proof.
+      induction 1.
+      { eexists; split.
+        + constructor.
+        + simpl. auto. }
+      { forward_reason.
+        eexists; split.
+        + constructor. eassumption.
+        + simpl. intros.
+          forward_reason; split; eauto. }
+      { forward_reason.
+        rewrite exprD'_conv
+          with (pfv:=eq_refl) (pfu:=f_equal _ (app_nil_r_trans _))
+            in H0.
+        autorewrite with eq_rw in H0. forwardy; inv_all; subst.
+        eexists; split.
+        + constructor. eassumption. eassumption.
+        + simpl. intros.
+          forward_reason; split; eauto.
+          rewrite H3; clear H3.
+          autorewrite with eq_rw.
+          f_equal.
+          rewrite hlist_app_nil_r.
+          clear.
+          generalize (app_nil_r_trans tus').
+          generalize (tus' ++ nil).
+          intros; subst. reflexivity. }
+    Qed.
+
+    Theorem mapD_nil_mapD_iff
+    : forall _tus _tus' _tvs tus tus' es R,
+        @mapD_nil _tus _tus' _tvs tus tus' es R ->
+        exists R',
+          @mapD _tus _tus' nil _tvs tus tus' es R' /\
+          forall _us _us' vs us us',
+            R _us _us' vs us us' <->
+            R' _us _us' vs us us' Hnil.
+    Proof.
+      induction 1.
+      { eexists; split.
+        + constructor.
+        + simpl. tauto. }
+      { forward_reason.
+        eexists; split.
+        + constructor. eassumption.
+        + simpl. intros.
+          rewrite H1. tauto. }
+      { forward_reason.
+        rewrite exprD'_conv
+          with (pfv:=eq_refl) (pfu:=f_equal _ (app_nil_r_trans _))
+            in H0.
+        autorewrite with eq_rw in H0. forwardy; inv_all; subst.
+        eexists; split.
+        + constructor. eassumption. eassumption.
+        + simpl. intros.
+          rewrite H2; clear H2.
+          eapply and_iff; try tauto.
+          autorewrite with eq_rw.
+          rewrite hlist_app_nil_r.
+          clear. generalize dependent (app_nil_r_trans tus').
+          generalize dependent (tus' ++ nil).
+          intros; subst; tauto. }
+    Qed.
 
     Lemma exprD'_UVar_ok
-      : forall tus tvs u t get,
+    : forall tus tvs u t get,
         nth_error_get_hlist_nth typD tus u = Some (@existT _ _ t get) ->
         exists eD,
           exprD' tus tvs (UVar u) t = Some eD /\
@@ -191,6 +306,32 @@ Section parameterized.
         forward_reason. inv_all. apply H0. assumption. }
     Qed.
 
+    Lemma lookup_compress_app
+    : forall xs ys b u,
+        lookup_compress (xs ++ ys) b u =
+        if u ?[ lt ] length xs then
+          lookup_compress xs b u
+        else
+          lookup_compress ys (b + length (filter (fun x => match x with
+                                                           | None => true
+                                                           | _ => false
+                                                           end) xs)) (u - length xs).
+    Proof.
+      clear.
+      induction xs; simpl.
+      { intros; f_equal.
+        symmetry; apply Plus.plus_0_r.
+        apply Minus.minus_n_O. }
+      { intros.
+        destruct u; try reflexivity.
+        replace (S u ?[ lt ] S (length xs)) with (u ?[ lt ] (length xs)).
+        destruct a.
+        { rewrite IHxs. forward. }
+        { rewrite IHxs. forward.
+          f_equal. simpl. omega. }
+        { reflexivity. } }
+    Qed.
+
     (** NOTE: This proof is ugly b/c of all of the extraction operations
      **)
     Lemma lookup_compress_sound
@@ -198,7 +339,7 @@ Section parameterized.
              (es : list (option expr))
              (R : hlist typD _tus -> hlist typD _tus' ->
                   hlist typD tvs -> hlist typD tus -> hlist typD tus' -> Prop),
-        mapD tus tus' es R ->
+        mapD_nil tus tus' es R ->
         forall (u : nat) (t : typ)
                (get : hlist typD (_tus ++ tus) -> typD t),
           nth_error_get_hlist_nth typD (_tus ++ tus) u =
@@ -216,8 +357,8 @@ Section parameterized.
       clear base_is_nus. clear c cs base.
       induction 1.
       { simpl; intros.
-        generalize (@UVar_exprD' typ expr _ _ _ _ (_tus' ++ tus) _tvs (length _tus' + (u - length _tus)) t).
-        destruct (exprD' (_tus' ++ tus) _tvs (UVar (length _tus' + (u - length _tus))) t).
+        generalize (@UVar_exprD' typ expr _ _ _ _ (_tus' ++ nil) _tvs (length _tus' + (u - length _tus)) t).
+        destruct (exprD' (_tus' ++ nil) _tvs (UVar (length _tus' + (u - length _tus))) t).
         { intros; forward_reason.
           eexists; split; eauto.
           eapply nth_error_get_hlist_nth_appR in H; [ | omega ].
@@ -254,7 +395,7 @@ Section parameterized.
           generalize (UVar_exprD' (_tus' ++ t :: tus') _tvs (length _tus') t0).
           destruct (exprD' (_tus' ++ t :: tus') _tvs (UVar (length _tus')) t0).
           { intros; forward_reason.
-            clear IHmapD.
+            clear IHmapD_nil.
             eapply nth_error_get_hlist_nth_appR in H2; [ | omega ].
             eapply nth_error_get_hlist_nth_appR in H0; [ | omega ].
             simpl in *. rewrite Minus.minus_diag in *.
@@ -268,7 +409,7 @@ Section parameterized.
             revert H6. rewrite (UIP_refl x2).
             intros; subst.
             assumption. }
-          { clear IHmapD.
+          { clear IHmapD_nil.
             eapply nth_error_get_hlist_nth_Some in H0; forward_reason.
             clear H0.
             intro XXX; exfalso; clear - x XXX; simpl in *.
@@ -277,15 +418,15 @@ Section parameterized.
             destruct XXX; forward_reason; try congruence. } }
         { intros.
           simpl.
-          specialize (IHmapD u).
-          repeat rewrite app_length in IHmapD. simpl in IHmapD.
-          replace (length _tus' + 1) with (S (length _tus')) in IHmapD by omega.
-          replace (u - (length _tus + 1)) with n in IHmapD by omega.
-          replace (length _tus + 1) with (S (length _tus)) in IHmapD by omega.
+          specialize (IHmapD_nil u).
+          repeat rewrite app_length in IHmapD_nil. simpl in IHmapD_nil.
+          replace (length _tus' + 1) with (S (length _tus')) in IHmapD_nil by omega.
+          replace (u - (length _tus + 1)) with n in IHmapD_nil by omega.
+          replace (length _tus + 1) with (S (length _tus)) in IHmapD_nil by omega.
           rewrite nth_error_get_hlist_nth_conv with (pf:=app_ass_trans _tus (t::nil) tus) in H0.
           autorewrite with eq_rw in H0. forward.
-          destruct s. specialize (IHmapD _ _ eq_refl).
-          destruct IHmapD; [ omega | omega | forward_reason ].
+          destruct s. specialize (IHmapD_nil _ _ eq_refl).
+          destruct IHmapD_nil; [ omega | omega | forward_reason ].
           inv_all; subst.
           rewrite exprD'_conv with (pfu:=app_ass_trans _tus' (t::nil) tus') (pfv:=eq_refl).
           revert H4. autorewrite with eq_rw. simpl.
@@ -305,7 +446,7 @@ Section parameterized.
         consider (u - length _tus).
         { intros.
           assert (u = length _tus) by omega.
-          subst. clear IHmapD H3 H4.
+          subst. clear IHmapD_nil H3 H4.
           eapply nth_error_get_hlist_nth_appR in H1; [ | omega ].
           simpl in H1. rewrite Minus.minus_diag in H1.
           forward_reason; inv_all; subst. subst.
@@ -316,12 +457,12 @@ Section parameterized.
         { intros.
           rewrite nth_error_get_hlist_nth_conv with (pf:=app_ass_trans _tus (t::nil) tus) in H1.
           autorewrite with eq_rw in H1.
-          specialize (IHmapD u).
+          specialize (IHmapD_nil u).
           forward.
           autorewrite with eq_rw in H5.
           inv_all; subst. subst.
           destruct s; simpl in *.
-          destruct (IHmapD _ _ eq_refl); clear IHmapD.
+          destruct (IHmapD_nil _ _ eq_refl); clear IHmapD_nil.
           { rewrite app_length; simpl; omega. }
           { rewrite app_length; simpl; omega. }
           forward_reason.
@@ -337,24 +478,81 @@ Section parameterized.
           reflexivity. } }
     Qed.
 
-    Lemma mapD_weaken_tvs : forall _tus _tus' _tvs _tvs' tus tus' es P,
-        @mapD _tus _tus' _tvs tus tus' es P ->
+    Lemma mapD_weaken_post
+    : forall _tus _tus' _tus_post _tus_post' _tvs tus tus' es P,
+        @mapD _tus _tus' _tus_post _tvs tus tus' es P ->
         exists P',
-          @mapD _tus _tus' (_tvs ++ _tvs') tus tus' es P' /\
-          forall U U' V V' a b,
-            P U U' V a b <-> P' U U' (hlist_app V V') a b.
-    Admitted.
+          @mapD _tus _tus' (_tus_post ++ _tus_post') _tvs tus tus' es P' /\
+          forall U U' c d V a b,
+            P U U' V a b c <-> P' U U' V a b (hlist_app c d).
+    Proof.
+      induction 1.
+      { eexists. split. econstructor. simpl. reflexivity. }
+      { forward_reason.
+        eexists; split. econstructor. eassumption.
+        simpl. intros.
+        rewrite H1. reflexivity. }
+      { forward_reason.
+        eapply exprD'_weaken with (tus':=_tus_post') (tvs' := nil) in H0;
+          eauto with typeclass_instances.
+        forward_reason.
+        rewrite exprD'_conv
+           with (pfv:=eq_refl) (pfu:=eq_sym (app_ass_trans _ _ _)) in H0.
+        rewrite exprD'_conv
+           with (pfv:=eq_sym (app_nil_r_trans _)) (pfu:=f_equal _ (eq_sym (app_ass_trans _ _ _))) in H0.
+        autorewrite with eq_rw in H0.
+        forwardy.
+        eexists; split. econstructor. eassumption.
+        eassumption. simpl. intros.
+        rewrite H2. inv_all. subst.
+        instantiate (1:=d).
+        erewrite H3 with (vs':=Hnil) (us':=d).
+        apply and_iff; [ | reflexivity ].
+        autorewrite with eq_rw.
+        rewrite hlist_app_assoc.
+        autorewrite with eq_rw.
+        rewrite hlist_app_nil_r.
+        autorewrite with eq_rw.
+        rewrite hlist_app_assoc.
+        generalize (hlist_app b (hlist_app c0 d)).
+        destruct (app_ass_trans tus' _tus_post'0 _tus_post').
+        reflexivity. }
+    Qed.
+
+    Lemma mapD_weaken_tvs
+    : forall _tus _tus' _tus_post _tvs _tvs' tus tus' es P,
+        @mapD _tus _tus' _tus_post _tvs tus tus' es P ->
+        exists P',
+          @mapD _tus _tus' _tus_post (_tvs ++ _tvs') tus tus' es P' /\
+          forall U U' c V V' a b,
+            P U U' V a b c <-> P' U U' (hlist_app V V') a b c.
+    Proof.
+      induction 1; simpl; intros.
+      { eexists. split. constructor.
+        simpl. intros; tauto. }
+      { forward_reason.
+        eexists; split.
+        - econstructor. eauto.
+        - simpl. intros. rewrite H1. reflexivity. }
+      { eapply exprD'_weakenV with (tvs':=_tvs') in H0; eauto.
+        forward_reason.
+        eexists; split.
+        - econstructor; eauto.
+        - simpl. intros.
+          rewrite <- H2. rewrite <- H3. reflexivity. }
+    Qed.
 
     Hypothesis WF_cs : WellFormed_ctx_subst cs.
 
     Lemma do_instantiate_sound
-      : forall (tus : list typ) (tvs : tenv typ) (tus' : list typ)
+      : forall (tus tvs tus' : tenv typ)
                (R : hlist typD (getUVars c) -> hlist typD (getUVars c) ->
-                    hlist typD tvs -> hlist typD tus -> hlist typD tus' -> Prop)
+                    hlist typD (getVars c ++ tvs) -> hlist typD tus ->
+                    hlist typD tus' -> Prop)
                (es : list (option expr)),
-        mapD tus tus' es R ->
+        @mapD_nil (getUVars c) (getUVars c) (getVars c ++ tvs) tus tus' es R ->
         forall sD,
-          ctx_substD (getUVars c) tvs cs = Some sD ->
+          ctx_substD (getUVars c) (getVars c) cs = Some sD ->
         forall (u : nat) (t : typ)
                (get : hlist typD (getUVars c ++ tus) -> typD t),
           nth_error_get_hlist_nth typD (getUVars c ++ tus) u =
@@ -363,21 +561,21 @@ Section parameterized.
                     get) ->
           match do_instantiate cs base es u with
             | Some eU =>
-              exists eUD : exprT (getUVars c ++ tus') tvs (typD t),
-                exprD' (getUVars c ++ tus') tvs eU t = Some eUD /\
+              exists eUD : exprT (getUVars c ++ tus') (_ ++ tvs) (typD t),
+                exprD' (getUVars c ++ tus') (getVars c ++ tvs) eU t = Some eUD /\
                 (forall (us : hlist typD (getUVars c ++ tus))
-                        (vs : hlist typD tvs) (us' : hlist typD (getUVars c ++ tus'))
+                        _vs (vs : hlist typD tvs) (us' : hlist typD (getUVars c ++ tus'))
                         (vs' : hlist typD tvs),
                     fst (hlist_split (getUVars c) tus us) =
                     fst (hlist_split (getUVars c) tus' us') /\
                     vs = vs' /\
                     R (fst (hlist_split (getUVars c) tus us))
                       (fst (hlist_split (getUVars c) tus us))
-                      vs
+                      (hlist_app _vs vs)
                       (snd (hlist_split (getUVars c) tus us))
                       (snd (hlist_split (getUVars c) tus' us')) ->
-                    sD (fst (hlist_split _ _ us)) vs ->
-                    get us = eUD us' vs')
+                    sD (fst (hlist_split _ _ us)) _vs ->
+                    get us = eUD us' (hlist_app _vs vs'))
             | None =>
               exists get' : hlist typD (getUVars c ++ tus') -> typD t,
                 nth_error_get_hlist_nth typD (getUVars c ++ tus') u =
@@ -386,17 +584,17 @@ Section parameterized.
                      (fun t0 : typ => hlist typD (getUVars c ++ tus') -> typD t0) t
                      get') /\
                 (forall (us : hlist typD (getUVars c ++ tus))
-                        (vs : hlist typD tvs) (us' : hlist typD (getUVars c ++ tus'))
+                        _vs (vs : hlist typD tvs) (us' : hlist typD (getUVars c ++ tus'))
                         (vs' : hlist typD tvs),
                     fst (hlist_split (getUVars c) tus us) =
                     fst (hlist_split (getUVars c) tus' us') /\
                     vs = vs' /\
                     R (fst (hlist_split (getUVars c) tus us))
                       (fst (hlist_split (getUVars c) tus us))
-                      vs
+                      (hlist_app _vs vs)
                       (snd (hlist_split (getUVars c) tus us))
                       (snd (hlist_split (getUVars c) tus' us')) /\
-                    sD (fst (hlist_split _ _ us)) vs ->
+                    sD (fst (hlist_split _ _ us)) _vs ->
                     get us = get' us')
           end.
     Proof.
@@ -404,10 +602,8 @@ Section parameterized.
       intros.
       generalize (lt_rem_sound base u).
       destruct (lt_rem u base); intros; forward_reason; subst.
-      { destruct (@lookup_compress_sound (getUVars c) (getUVars c) tus tus' tvs es _ H u _ _ H1).
-        { Instance Reflexive_ge : Reflexive ge.
-          Proof. constructor. Qed.
-          reflexivity. }
+      { destruct (@lookup_compress_sound (getUVars c) (getUVars c) tus tus' (_ ++ tvs) es _ H u _ _ H1).
+        { reflexivity. }
         { assumption. }
         { forward_reason.
           eexists; split; eauto.
@@ -424,15 +620,15 @@ Section parameterized.
           intros; forward_reason.
           destruct (@nth_error_get_hlist_nth_appL _ typD tus _ _ H2).
           rewrite H1 in H7. forward_reason; inv_all; subst; simpl in *.
-          eapply exprD'_weakenU with (tus':=tus') in H5; try eassumption.
+          eapply exprD'_weaken with (tus':=tus') (tvs':=tvs) in H5; try eassumption.
           destruct H5 as [ ? [ ? ? ] ].
           rewrite H4 in H8. inv_all; subst.
           eexists; split; eauto.
           intros. forward_reason. subst.
           specialize (H6 _ _ H10).
           clear - H7 H9 H6 H8.
-          specialize (H7 (fst (hlist_split _ _ us)) vs'
-                         (snd (hlist_split _ _ us'))).
+          specialize (H7 (fst (hlist_split _ _ us)) _vs
+                         (snd (hlist_split _ _ us')) vs').
           specialize (H9 (fst (hlist_split _ _ us)) (snd (hlist_split _ _ us))).
           rewrite hlist_app_hlist_split in H9.
           rewrite H8 in *.
@@ -454,40 +650,41 @@ Section parameterized.
           intros. rewrite H0. symmetry; eassumption. } }
     Qed.
 
-    Lemma instantiate_do_instantiate_sound
+    Lemma instantiate_do_instantiate_exprD'_sound
     : forall (tus : list typ) (tvs : tenv typ) (tus' : list typ)
-             (e : expr)
+             (e : expr) t
              (R : hlist typD (getUVars c) -> hlist typD (getUVars c) ->
-                  hlist typD tvs -> hlist typD tus -> hlist typD tus' -> Prop)
+                  hlist typD _ -> hlist typD tus -> hlist typD tus' -> Prop)
              (es : list (option expr)),
-        mapD tus tus' es R ->
+        @mapD_nil (getUVars c) (getUVars c) (getVars c ++ tvs) tus tus' es R ->
         forall sD,
-          ctx_substD (getUVars c) tvs cs = Some sD ->
-        forall gD : exprT (getUVars c ++ tus) tvs Prop,
-          propD (getUVars c ++ tus) tvs e = Some gD ->
-          exists gD' : exprT (getUVars c ++ tus') tvs Prop,
-            propD (getUVars c ++ tus') tvs
-                  (instantiate (do_instantiate cs base es) 0 e) =
+          ctx_substD (getUVars c) (getVars c) cs = Some sD ->
+        forall gD : exprT (getUVars c ++ tus) _ _,
+          exprD' (getUVars c ++ tus) (getVars c ++ tvs) e t = Some gD ->
+          exists gD' : exprT (getUVars c ++ tus') (getVars c ++ tvs) _,
+            exprD' (getUVars c ++ tus') (getVars c ++ tvs)
+                  (instantiate (do_instantiate cs base es) 0 e) t =
             Some gD' /\
-            (forall (_us : hlist typD (getUVars c)) (_vs : hlist typD tvs)
+            (forall (_us : hlist typD (getUVars c)) _vsx (_vs : hlist typD tvs)
                     (us : hlist typD tus) (us' : hlist typD tus'),
-                R _us _us _vs us us' ->
-                sD _us _vs ->
-                (gD' (hlist_app _us us') _vs <-> gD (hlist_app _us us) _vs)).
+                R _us _us (hlist_app _vsx _vs) us us' ->
+                sD _us _vsx ->
+                (gD' (hlist_app _us us') (hlist_app _vsx _vs) =
+                 gD (hlist_app _us us) (hlist_app _vsx _vs))).
     Proof.
-      unfold propD, exprD'_typ0.
       intros; forward; inv_all.
-      pose (R':=fun us vs us' vs' =>
+      pose (R':=fun (us : hlist _ (getUVars c ++ tus)) (vs : hlist _ (getVars c ++ tvs))
+                    (us' : hlist _ (getUVars c ++ tus')) (vs' : hlist _ (getVars c ++ tvs)) =>
                  fst (hlist_split _ _ us) = fst (hlist_split _ _ us') /\
                  vs = vs' /\
                  R (fst (hlist_split _ _ us)) (fst (hlist_split _ _ us)) vs (snd (hlist_split _ _ us)) (snd (hlist_split _ _ us')) /\
-                 sD (fst (hlist_split _ _ us)) vs).
+                 sD (fst (hlist_split _ _ us)) (fst (hlist_split _ _ vs))).
       destruct (fun Hu Hv => @expr_subst_sound _ _ _ _ _
-                    (do_instantiate cs (length (getUVars c)) es) (fun _ => None) 0 e _ eq_refl
-                    nil (getUVars c ++ tus) tvs (getUVars c ++ tus') tvs
+                    (do_instantiate cs (length (getUVars c)) es) (fun _ => None) _ e _ eq_refl
+                    nil (getUVars c ++ tus) (getVars c ++ tvs) (getUVars c ++ tus') (getVars c ++ tvs)
                     R'
                     Hu Hv
-                    (typ0 (F:=Prop)) _ eq_refl H1).
+                    t _ eq_refl H1).
       { (* Hu *)
         intros.
         generalize (@do_instantiate_sound _ _ _ _ _ H _ H0 _ _ _ H3).
@@ -497,133 +694,1023 @@ Section parameterized.
           eexists; split; eauto.
           subst R'. simpl. intros.
           forward_reason.
-          eapply H4. eauto. eauto. }
-        { unfold R'. eauto. } }
+          rewrite <- (hlist_app_hlist_split _ _ vs').
+          eapply H5.
+          split; eauto. split; eauto.
+          rewrite hlist_app_hlist_split. subst. auto.
+          subst. auto. }
+        { unfold R'.
+          clear. destruct 1.
+          exists x.
+          forward_reason; split; eauto.
+          intros. forward_reason. eapply H0.
+          split. eassumption.
+          split.
+          2: split; try eassumption.
+          2: rewrite hlist_app_hlist_split; eassumption.
+          reflexivity. } }
       { (* Hv *)
         intros; eexists; split; eauto.
         subst R'. simpl. intros. forward_reason.
         subst. reflexivity. }
       { forward_reason.
-        subst. change_rewrite H3.
+        subst. change_rewrite H2.
         eexists; split; eauto.
         intros.
-        specialize (H4 (hlist_app _us us) _vs (hlist_app _us us') _vs Hnil).
-        subst R'. simpl in H4.
-        repeat rewrite hlist_split_hlist_app in H4. simpl in H4.
-        autorewrite with eq_rw. rewrite H4.
+        specialize (H3 (hlist_app _us us) (hlist_app _vsx _vs) (hlist_app _us us') (hlist_app _vsx _vs) Hnil).
+        subst R'. simpl in H3.
+        repeat rewrite hlist_split_hlist_app in H3. simpl in H3.
+        autorewrite with eq_rw. rewrite H3.
         reflexivity. eauto. }
     Qed.
 
-    (** TODO(gmalecha): move to bimap **)
-    Lemma only_in_range_empty : forall a b,
-        only_in_range a b (amap_empty expr).
+    Corollary instantiate_do_instantiate_propD_sound
+    : forall (tus : list typ) (tvs : tenv typ) (tus' : list typ)
+             (e : expr)
+             (R : hlist typD (getUVars c) -> hlist typD (getUVars c) ->
+                  hlist typD (getVars c ++ tvs) -> hlist typD tus -> hlist typD tus' -> Prop)
+             (es : list (option expr)),
+        mapD_nil tus tus' es R ->
+        forall sD,
+          ctx_substD (getUVars c) (getVars c) cs = Some sD ->
+        forall gD : exprT (getUVars c ++ tus) _ Prop,
+          propD (getUVars c ++ tus) (getVars c ++ tvs) e = Some gD ->
+          exists gD' : exprT (getUVars c ++ tus') _ Prop,
+            propD (getUVars c ++ tus') (getVars c ++ tvs)
+                  (instantiate (do_instantiate cs base es) 0 e) =
+            Some gD' /\
+            (forall (_us : hlist typD (getUVars c)) _vsx (_vs : hlist typD _)
+                    (us : hlist typD tus) (us' : hlist typD tus'),
+                R _us _us (hlist_app _vsx _vs) us us' ->
+                sD _us _vsx ->
+                (gD' (hlist_app _us us') (hlist_app _vsx _vs) <->
+                 gD (hlist_app _us us) (hlist_app _vsx _vs))).
     Proof.
-      clear. red. intros.
-      eapply Forall_amap_empty.
-    Qed.
-
-    Lemma WellFormed_amap_amap_empty : WellFormed_amap (amap_empty expr).
-    Proof. red. eapply FMapSubst.SUBST.WellFormed_empty. Qed.
-
-    Lemma mapD_conv
-    : forall a b c us us' vs vs' es es' R
-             (pf_us:us=us') (pf_vs:vs=vs'),
-        es = es' ->
-        (@mapD a b c us vs es R <->
-         @mapD a b c us' vs' es'
-               match pf_us in _ = us
-                   , pf_vs in _ = vs
-                     return hlist _ a -> hlist _ b -> hlist _ c ->
-                            hlist _ us -> hlist _ vs -> Prop
-               with
-                 | eq_refl , eq_refl => R
-               end).
-    Proof.
-      clear. destruct pf_us. destruct pf_vs. intros; subst.
+      unfold propD, exprD'_typ0.
+      intros; forward; inv_all.
+      eapply instantiate_do_instantiate_exprD'_sound in H1; eauto.
+      forward_reason.
+      rewrite H1. eexists; split; eauto.
+      intros. eapply H3 in H4; eauto.
+      subst.
+      autorewrite with eq_rw.
+      rewrite H4.
       reflexivity.
     Qed.
 
-    (** What is missing here is the fact that [amap_substD a]
-     ** is equivalent to [list_substD tus tvs start ls]
-     **)
-    Theorem amap_substD_list_substD
-      : forall tus tvs am (from len : nat) sD maxV,
-        WellFormed_bimap from len maxV am ->
-        amap_substD tus tvs am = Some sD ->
-        exists sD',
-          FMapSubst.SUBST.list_substD tus tvs from (amap_aslist am from len) = Some sD' /\
-          forall us vs,
-            sD us vs <-> sD' us vs.
+    Lemma mapD_conv
+    : forall a b c vs vs' us us' _us _us' es es' R
+             (pf_vs:vs=vs') (pf_us:us=us') (pf_us':_us=_us'),
+        es = es' ->
+        (@mapD a b c vs  us _us es R <->
+         @mapD a b c vs' us' _us' es'
+               match pf_vs in _ = vs
+                   , pf_us in _ = us
+                   , pf_us' in _ = us'
+                     return hlist _ a -> hlist _ b -> hlist _ vs ->
+                            hlist _ us -> hlist _ us' -> hlist _ _ -> Prop
+               with
+                 | eq_refl , eq_refl , eq_refl => R
+               end).
     Proof.
-      destruct 1.
-      intros; eapply FMapSubst.SUBST.amap_substD_list_substD; eauto.
-      destruct H0. eauto.
+      clear. destruct pf_us. destruct pf_vs. destruct pf_us'. intros; subst.
+      reflexivity.
     Qed.
 
-    Lemma minify_goal_sound
+    Lemma mapD_nil_conv
+    : forall a a' b b' vs vs' us us' _us _us' es es' R
+             (pf__us : a = a') (pf__us' : b = b') (pf_vs:vs=vs') (pf_us:us=us') (pf_us':_us=_us'),
+        es = es' ->
+        (@mapD_nil a b vs  us _us es R <->
+         @mapD_nil a' b' vs' us' _us' es'
+               match pf__us in _ = a
+                   , pf__us' in _ = b
+                   , pf_vs in _ = vs
+                   , pf_us in _ = us
+                   , pf_us' in _ = us'
+                     return hlist _ a -> hlist _ b -> hlist _ vs ->
+                            hlist _ us -> hlist _ us' -> Prop
+               with
+                 | eq_refl , eq_refl , eq_refl , eq_refl , eq_refl => R
+               end).
+    Proof.
+      clear. intros; subst. reflexivity.
+    Qed.
+
+
+
+    Lemma mapD_app_lem
+    : forall tus_base tus_base' tvs tus tus',
+      forall es _post R,
+        @mapD tus_base tus_base' _post tvs tus tus' es R ->
+        forall ts ts' mlist_inst _tus_post R',
+          @mapD (tus_base ++ tus) (tus_base' ++ tus') _tus_post tvs ts ts' mlist_inst R' ->
+          forall (pf : ts' ++ _tus_post = _post),
+          exists R'',
+            @mapD tus_base tus_base' _tus_post tvs (tus ++ ts) (tus' ++ ts') (es ++ mlist_inst) R'' /\
+            forall _us _us' vs us us' us'',
+              R'' _us _us' vs us us' us'' <->
+              (R _us _us' vs (fst (hlist_split _ _ us)) (fst (hlist_split _ _ us'))
+                 match pf in _ = t return hlist _ t with
+                 | eq_refl => hlist_app (snd (hlist_split _ _ us')) us''
+                 end /\
+               R' (hlist_app _us (fst (hlist_split _ _ us)))
+                  (hlist_app _us' (fst (hlist_split _ _ us')))
+                  vs (snd (hlist_split _ _ us)) (snd (hlist_split _ _ us')) us'').
+    Proof. clear.
+      induction 1.
+      { simpl; intros ? ? ?.
+        intros. setoid_rewrite hlist_app_nil_r.
+        revert H; revert R'.
+        generalize dependent (eq_sym (app_nil_r_trans _tus)).
+        generalize dependent (eq_sym (app_nil_r_trans _tus')).
+        generalize (_tus ++ nil); generalize (_tus' ++ nil); intros; subst.
+        eexists; split; eauto.
+        intros. intuition. }
+      { Opaque hlist_split.
+        simpl; intros; subst.
+        cut (@mapD ((_tus ++ t :: nil) ++ tus) ((_tus' ++ t :: nil) ++ tus') _tus_post _tvs ts ts' mlist_inst
+                   match eq_sym (app_ass_trans _ _ _) in _ = t
+                       , eq_sym (app_ass_trans _ _ _) in _ = t'
+                         return hlist _ t -> hlist _ t' -> _
+                   with
+                     | eq_refl , eq_refl => R'
+                   end).
+        { clear H0. intros.
+          eapply IHmapD in H0; clear IHmapD.
+          forward_reason.
+          eexists; split.
+          { simpl. constructor. eassumption. }
+          simpl. intros.
+          rewrite H1; clear H1. clear.
+          Transparent hlist_split. simpl.
+          change (fix app (l m : list typ) {struct l} :
+                    list typ :=
+                      match l with
+                      | nil => m
+                      | a0 :: l1 => a0 :: app l1 m
+                      end) with (@app typ).
+          destruct (@hlist_split typ (@typD typ RType_typ) tus ts
+                                 (@hlist_tl typ (@typD typ RType_typ) t
+                                            (tus ++ ts) us)).
+          destruct (@hlist_split typ (@typD typ RType_typ) tus' ts'
+                                 (@hlist_tl typ (@typD typ RType_typ) t
+                                            (tus' ++ ts') us')).
+          simpl. autorewrite with eq_rw.
+          do 2 rewrite hlist_app_assoc.
+          autorewrite with eq_rw.
+          simpl. instantiate (1 := eq_refl).
+          repeat rewrite <- and_assoc.
+          eapply and_iff. reflexivity.
+          intro. rewrite H0.
+          tauto. }
+        { revert H0. clear.
+          destruct (@eq_sym (list typ) ((_tus ++ t :: @nil typ) ++ tus)
+                            (_tus ++ (t :: @nil typ) ++ tus)
+                            (@app_ass_trans typ _tus (t :: @nil typ) tus)).
+          destruct (@eq_sym (list typ) ((_tus' ++ t :: @nil typ) ++ tus')
+                            (_tus' ++ (t :: @nil typ) ++ tus')
+                            (@app_ass_trans typ _tus' (t :: @nil typ) tus')).
+          exact (fun x => x). } }
+      { intros. subst.
+        cut (@mapD ((_tus ++ t :: nil) ++ tus) (_tus' ++ tus') _tus_post _tvs ts ts' mlist_inst
+                   match eq_sym (app_ass_trans _ _ _) in _ = t
+                         return hlist _ t -> hlist _ _ -> _
+                   with
+                     | eq_refl => R'
+                   end).
+        { clear H; intros.
+          eapply IHmapD in H; clear IHmapD.
+          forward_reason. subst.
+          rewrite exprD'_conv
+             with (pfu:=f_equal _ (app_ass_trans _ _ _)) (pfv:=eq_refl)
+               in H0.
+          autorewrite with eq_rw in H0. forwardy.
+          inv_all; subst.
+          eexists; split.
+          { simpl. constructor. eauto. eauto. }
+          Opaque hlist_split.
+          simpl. intros.
+          rewrite H2; clear H2.
+          autorewrite with eq_rw.
+          rewrite <- and_assoc.
+          eapply and_iff.
+          { rewrite (hlist_eta us); simpl.
+            rewrite hlist_hd_fst_hlist_split. simpl.
+            rewrite (hlist_app_assoc' (fst _) (snd _) _).
+            rewrite hlist_app_hlist_split.
+            clear.
+            destruct (app_ass_trans tus' ts' _tus_post). reflexivity. }
+          intros. eapply and_iff.
+          { rewrite hlist_hd_fst_hlist_split.
+            rewrite hlist_tl_fst_hlist_split.
+            instantiate (1:=eq_refl).
+            reflexivity. }
+          intros.
+          rewrite hlist_app_assoc. autorewrite with eq_rw.
+          rewrite hlist_tl_snd_hlist_split.
+          eapply iff_eq. f_equal.
+          rewrite (hlist_eta us). simpl.
+          Transparent hlist_split. simpl.
+          match goal with
+          | |- context [ match ?X with _ => _ end ] =>
+            destruct X
+          end. reflexivity. }
+        { revert H1. clear.
+          revert R'.
+          destruct (eq_sym (app_ass_trans _tus (t :: nil) tus)). tauto. } }
+    Qed.
+
+    Lemma list_substD_conv
+    : forall tus tus' tvs tvs' n n' (s : list (option expr))
+             (pfu : tus=tus') (pfv:tvs=tvs') (pfn : n=n'),
+        FMapSubst.SUBST.list_substD tus tvs n s =
+        match eq_sym pfu in _ = t
+                            , eq_sym pfv in _ = t' return option (exprT t t' Prop) with
+        | eq_refl , eq_refl => FMapSubst.SUBST.list_substD tus' tvs' n' s
+        end.
+    Proof.
+      destruct pfu; destruct pfv; destruct 1; eauto.
+    Qed.
+
+    Lemma length_list_subst
+    : forall a N b mlist,
+        mlist = amap_aslist (expr:=expr) a b N ->
+        length mlist = N.
+    Proof.
+      clear. induction N; simpl; intros; subst; auto.
+      simpl. f_equal. eapply IHN. reflexivity.
+    Qed.
+
+    Lemma types_after_instantiate_map_fmap
+    : forall f ts es,
+        types_after_instantiate ts (map (Functor.fmap f) es) =
+        types_after_instantiate ts es.
+    Proof.
+      induction ts; destruct es; simpl; auto.
+      { destruct o; eauto.
+        f_equal. eauto. }
+    Qed.
+
+    Lemma mapD_nil_ex
+    : forall _tus _tus' tvs ts mlist R,
+        @mapD_nil _tus _tus' tvs ts (types_after_instantiate ts mlist) mlist R ->
+        forall _us _us' vs (us' : hlist _ (types_after_instantiate ts mlist)),
+        exists us,
+          R _us _us' vs us us'.
+    Proof.
+      clear. induction 1.
+      { eauto. }
+      { intros.
+        destruct (IHmapD_nil (hlist_app _us (Hcons (hlist_hd us') Hnil))
+                             (hlist_app _us' (Hcons (hlist_hd us') Hnil))
+                             vs (hlist_tl us')).
+        exists (Hcons (hlist_hd us') x).
+        simpl. eauto. }
+      { intros.
+        destruct (IHmapD_nil (hlist_app _us (Hcons (eD (hlist_app _us' us') vs) Hnil))
+                             _us' vs us').
+        exists (Hcons (eD (hlist_app _us' us') vs) x).
+        simpl. eauto. }
+    Qed.
+
+    Lemma mapD_nil_app
+    : forall tus_base tus_base' tvs tus tus' es R,
+        @mapD_nil tus_base tus_base' tvs tus tus' es R ->
+        forall ts ts' mlist_inst R',
+          @mapD_nil (tus_base ++ tus) (tus_base' ++ tus') tvs ts ts' mlist_inst R' ->
+          exists R'',
+            @mapD_nil tus_base tus_base' tvs (tus ++ ts) (tus' ++ ts') (es ++ mlist_inst) R'' /\
+            forall __us __us' _us _us' vs us us',
+              R'' __us __us' vs (hlist_app _us us) (hlist_app _us' us') <->
+              (   R __us __us' vs _us _us'
+                  /\ R' (hlist_app __us _us) (hlist_app __us' _us') vs us us').
+    Proof.
+      induction 1; simpl; intros.
+      { intros.
+        exists (match app_nil_r_trans _tus in _ = _tu
+                    , app_nil_r_trans _tus' in _ = _tu'
+                      return hlist _ _tu -> hlist _ _tu' -> _
+                with
+                | eq_refl , eq_refl => R'
+                end).
+        split.
+        { destruct (app_nil_r_trans _tus).
+          destruct (app_nil_r_trans _tus'). assumption. }
+        { intros.
+          rewrite (hlist_eta _us).
+          rewrite (hlist_eta _us'). simpl.
+          rewrite hlist_app_nil_r. rewrite hlist_app_nil_r.
+          clear.
+          generalize dependent (app_nil_r_trans _tus).
+          generalize dependent (app_nil_r_trans _tus').
+          generalize dependent (_tus' ++ nil).
+          generalize dependent (_tus ++ nil).
+          intros; subst. tauto. } }
+      { apply (@mapD_nil_conv _ _ _ _ _tvs _ ts _ ts' _ mlist_inst _ R' (eq_sym (app_ass_trans _ (t::nil) _)) (eq_sym (app_ass_trans _ (t::nil) _)) eq_refl eq_refl eq_refl eq_refl) in H0.
+        eapply IHmapD_nil in H0.
+        forward_reason.
+        eexists; split.
+        { constructor; eauto. }
+        { simpl. intros.
+          specialize (H1 (hlist_app __us (Hcons (hlist_hd _us) Hnil))
+                         (hlist_app __us' (Hcons (hlist_hd _us') Hnil))
+                         (hlist_tl _us) (hlist_tl _us') vs us us').
+          rewrite (hlist_eta _us). simpl.
+          rewrite (hlist_eta _us'). simpl.
+          rewrite <- and_assoc.
+          apply and_iff. reflexivity. intros.
+          destruct H2. rewrite H1.
+          clear.
+          rewrite hlist_app_assoc.
+          rewrite hlist_app_assoc.
+          generalize (app_ass_trans _tus (t :: nil) tus).
+          generalize (app_ass_trans _tus' (t :: nil) tus').
+          simpl.
+          generalize ((_tus' ++ t :: nil) ++ tus').
+          generalize ((_tus ++ t :: nil) ++ tus).
+          intros; subst. simpl.
+          tauto. } }
+      { apply (@mapD_nil_conv _ _ _ _ _tvs _ ts _ ts' _ mlist_inst _ R' (eq_sym (app_ass_trans _ (t::nil) _)) eq_refl eq_refl eq_refl eq_refl eq_refl) in H1.
+        eapply IHmapD_nil in H1; clear IHmapD_nil.
+        forward_reason.
+        eapply exprD'_weakenU with (tus':=ts') in H0; [ | eauto ].
+        forward_reason.
+        rewrite exprD'_conv
+           with (pfu:=eq_sym (app_ass_trans _ _ _)) (pfv:=eq_refl)
+             in H0.
+        autorewrite with eq_rw in H0.
+        forwardy. inv_all; subst.
+        eexists; split.
+        { econstructor; eauto. }
+        { simpl. intros.
+          rewrite <- and_assoc.
+          eapply and_iff.
+          { rewrite (hlist_eta _us). simpl.
+            rewrite hlist_app_assoc'.
+            erewrite H3.
+            instantiate (1 := us').
+            clear. destruct (app_ass_trans _tus' tus' ts').
+            tauto. }
+          { intro.
+            clear - H2.
+            specialize (H2 (hlist_app __us (Hcons (hlist_hd _us) Hnil))
+                           __us' (hlist_tl _us) _us' vs us us').
+            rewrite (hlist_eta _us). simpl.
+            rewrite H2. clear.
+            apply and_iff. reflexivity. intro.
+            rewrite hlist_app_assoc.
+            autorewrite with eq_rw. tauto. } } }
+    Qed.
+
+    Lemma types_after_instantiate_Some_end
+    : forall c t a b,
+        length a = length b ->
+        types_after_instantiate a b =
+        types_after_instantiate (a ++ t :: nil) (b ++ Some c :: nil).
+    Proof.
+      induction a; destruct b; simpl; intros; auto.
+      { inversion H. }
+      { inversion H. }
+      { rewrite IHa. reflexivity. omega. }
+    Qed.
+
+
+    Lemma types_after_instantiate_firstn_skipn
+      : forall n ts es,
+        types_after_instantiate (firstn n ts) (firstn n es) ++
+                                types_after_instantiate (skipn n ts) (skipn n es) =
+        types_after_instantiate ts es.
+    Proof.
+      induction n; simpl; intros; auto.
+      { destruct ts; simpl.
+        + destruct es; try reflexivity.
+          destruct (skipn n es); reflexivity.
+        + destruct es; [ | destruct o; simpl; try rewrite IHn ; reflexivity ].
+          destruct (skipn n ts); reflexivity. }
+    Qed.
+
+    Ltac inst_hlists :=
+      repeat match goal with
+             | h : hlist _ _ , H : forall x : hlist _ _, _ |- _ =>
+               first [ specialize (H h)
+                     | specialize (H (fst (hlist_split _ _ h))) ]
+             | h : hlist _ _ , h' : hlist _ _ , H : forall x : hlist _ _, _  |- _ =>
+               specialize (H (hlist_app h h'))
+             | h : hlist _ _ , h' : hlist _ _ , h'' : hlist _ _ , H : forall x : hlist _ _, _ |- _ =>
+               first [ specialize (H (hlist_app h (hlist_app h' h'')))
+                     | specialize (H (hlist_app (hlist_app h h') h'')) ]
+             end.
+
+
+    Fixpoint Forgetting ts (es : list (option expr))
+      : hlist typD ts -> hlist typD (types_after_instantiate ts es) -> Prop :=
+      match ts as ts , es as es
+            return hlist typD ts -> hlist typD (types_after_instantiate ts es) -> Prop
+      with
+      | nil , nil => @eq _
+      | nil , _ :: _ => @eq _
+      | t :: ts , None :: es => fun a b => hlist_hd a = hlist_hd b
+                                           /\ @Forgetting ts es (hlist_tl a) (hlist_tl b)
+      | t :: ts , Some _ :: es => fun a b => @Forgetting ts es (hlist_tl a) b
+      | _ :: _ , nil => fun _ _ => False
+      end.
+
+    Fixpoint Forget ts (es : list (option expr))
+    : hlist typD ts -> hlist typD (types_after_instantiate ts es) :=
+      match ts as ts , es as es
+            return hlist typD ts -> hlist typD (types_after_instantiate ts es)
+      with
+      | nil , nil => fun x => x
+      | nil , _ :: _ => fun x => x
+      | t :: ts , nil => fun _ => Hnil
+      | t :: ts , None :: es => fun x =>
+                                  Hcons (hlist_hd x) (@Forget ts es (hlist_tl x))
+      | t :: ts , Some _ :: es => fun x => @Forget ts es (hlist_tl x)
+      end.
+
+    Lemma mapD_nil_Forgetting'
+    : forall a b c d e f R,
+        @mapD_nil a b c d e f R ->
+        forall A B C D E,
+          R A B C D E ->
+          exists pf : e = types_after_instantiate d f,
+            Forgetting f D match pf in _ = t return hlist _ t with
+                           | eq_refl => E
+                           end.
+    Proof.
+      clear. induction 1; simpl; intros; subst.
+      { exists eq_refl. reflexivity. }
+      { forward_reason.
+        eapply IHmapD_nil in H1.
+        forward_reason. exists (f_equal _ x).
+        subst. eauto. }
+      { forward_reason.
+        eapply IHmapD_nil in H2.
+        forward_reason. subst.
+        exists eq_refl. auto. }
+    Qed.
+
+    Lemma mapD_nil_Forgetting
+    : forall a b c d f R,
+        @mapD_nil a b c d _ f R ->
+        forall A B C D E,
+          R A B C D E ->
+          Forgetting f D E.
+    Proof.
+      intros.
+      generalize (@mapD_nil_Forgetting' a b c0 d _ f R H _ _ _ _ _ H0).
+      intros; forward_reason.
+      cutrewrite (x = eq_refl) in H1; auto.
+      unfold tenv in *.
+      apply UIP_refl.
+    Qed.
+
+    Lemma the_actual_lemma
+    : forall f (_tus _tus' tvs : tenv typ) (a : amap expr)
+        (WFa : FMapSubst.SUBST.WellFormed a),
+        forall (tus_ tus tus' : tenv typ) mlist1_inst
+          (Hlen : length mlist1_inst = length tus),
+          let mlist2 := amap_aslist a (length (_tus ++ tus)) (length tus_) in
+          let mlist2_inst := map (Functor.fmap f) mlist2 in
+          forall R sD' P
+            (HmapD : @mapD _tus
+                  _tus'
+                  (types_after_instantiate tus_ mlist2)
+                  tvs
+                  tus
+                  tus'
+                  mlist1_inst R)
+            (HsubstD : FMapSubst.SUBST.list_substD
+              (_tus ++ tus ++ tus_)
+              tvs
+              (length (_tus ++ tus))
+              mlist2 = Some sD')
+            (Hf : forall (n : nat) e t eD,
+                nth_error mlist2 n = Some (Some e) ->
+                exprD' (_tus ++ tus ++ tus_) tvs e t = Some eD ->
+                exists eD',
+                  exprD' (_tus' ++ tus' ++
+                          types_after_instantiate tus_ mlist2)
+                         tvs (f e) t = Some eD' /\
+                  forall _us _us' vs us us' us_ us_',
+                    forall HP : P _us _us' vs,
+                    forall Hfor : Forgetting mlist2 us_ us_',
+                    R _us _us' vs us us' us_' ->
+                    eD (hlist_app _us (hlist_app us us_)) vs =
+                    eD' (hlist_app _us' (hlist_app us' us_')) vs),
+            exists R',
+              @mapD_nil _tus _tus' tvs (tus ++ tus_)
+                        (tus' ++
+                         types_after_instantiate tus_ mlist2)
+                        (mlist1_inst ++ mlist2_inst)  R' /\
+              forall _us _us' vs us us' us_',
+                forall (HP : P _us _us' vs),
+                R _us _us' vs us us' us_' ->
+                exists us_,
+                  Forgetting mlist2 us_ us_' /\
+                  sD' (hlist_app _us (hlist_app us us_)) vs /\
+                  R' _us _us' vs (hlist_app us us_) (hlist_app us' us_').
+    Proof.
+      clear. induction tus_; intros.
+      { simpl. simpl in *.
+        eapply mapD_mapD_nil in HmapD.
+        forward_reason.
+        eapply mapD_nil_conv
+          with (pf_us:=eq_sym (app_nil_r_trans _))
+               (pf_us':=eq_sym (app_nil_r_trans _))
+               (pf_vs:=eq_refl)
+               (pf__us:=eq_refl) (pf__us':=eq_refl) in H.
+        eexists; split.
+        { eapply H. }
+        { clear H.
+          intros.
+          inv_all. subst. exists Hnil.
+          rewrite (hlist_eta us_').
+          split; auto. split; auto.
+          autorewrite with eq_rw.
+          do 2 rewrite hlist_app_nil_r.
+          autorewrite with eq_rw.
+          eapply H0. eauto. }
+        { unfold mlist2_inst. symmetry. apply app_nil_r_trans. } }
+      { simpl in *. subst mlist2. subst mlist2_inst.
+        consider (amap_lookup (length (_tus ++ tus)) a);
+          intros; forwardy; inv_all; subst.
+        { eapply nth_error_get_hlist_nth_appR in H0;
+          [ simpl in H0; forward_reason | repeat rewrite app_length; simpl; omega ].
+          eapply nth_error_get_hlist_nth_appR in H0;
+          [ simpl in H0; forward_reason | repeat rewrite app_length; simpl; omega ].
+          rewrite app_length in H0.
+          replace (length _tus + length tus - length _tus - length tus) with 0 in H0 by omega.
+          inv_all. subst.
+          specialize (IHtus_ (tus ++ a0 :: nil) tus' (mlist1_inst ++ Some (f e) :: nil)).
+          eapply Hf in H1. 2: instantiate (1 :=0); reflexivity.
+          destruct H1 as [ eD' [ HeD' HeD'eq ] ].
+          rewrite exprD'_conv
+            with (pfu:=app_ass_trans _ _ _) (pfv:=eq_refl) in HeD'.
+          autorewrite with eq_rw in HeD'. forwardy.
+          edestruct (@mapD_app_lem _ _ _ _ _ _ _ _ HmapD (a0 :: nil) nil (Some (f e) :: nil)).
+          { constructor. constructor. simpl. eassumption. }
+          revert H6; instantiate (1 := eq_refl); intro H6.
+          destruct H6 as [ HmapD' ? ].
+          assert (Heq : S (@length typ (_tus ++ tus)) = length (_tus ++ tus ++ a0 :: nil)).
+          { repeat rewrite app_length. simpl. omega. }
+          destruct Heq.
+          eapply mapD_conv
+              with (pf_vs:=eq_refl)
+                   (pf_us:=eq_refl) (pf_us':=app_nil_r_trans _)
+              in HmapD'; [ | reflexivity ].
+          erewrite list_substD_conv
+               with (pfu:=eq_sym (f_equal (app _) (app_ass_trans tus (a0::nil) tus_)))
+                    (pfv:=eq_refl)
+              in H2; [ | reflexivity ].
+          simpl in H2.
+          autorewrite with eq_rw in H2. forwardy.
+          edestruct IHtus_ with (P:=P).
+          { repeat rewrite app_length. simpl. omega. }
+          { eapply HmapD'. }
+          { eapply H2. }
+          { inv_all. subst. clear - Hf H H3 H4 H6.
+            do 4 intro. intro Hnth. intro H0.
+            rewrite exprD'_conv
+              with (pfu:=f_equal _ (eq_sym (app_ass_trans _ _ _))) (pfv:=eq_refl) in H0.
+            simpl in H0. autorewrite with eq_rw in H0.
+            forwardy.
+            eapply Hf in H0; clear Hf. 2: instantiate (1 := S n); eassumption.
+            inv_all. subst.
+            destruct H0 as [ ? [ ? ? ] ].
+            eexists; split; eauto.
+            intros.
+            inst_hlists.
+            autorewrite with eq_rw in H2.
+            eapply H6 in H2; clear H6.
+            specialize (H1 (hlist_app (snd (hlist_split _ _ us)) us_) us_').
+            rewrite <- H1; try eassumption.
+            { autorewrite with eq_rw.
+              generalize (hlist_app_assoc' (fst (hlist_split _ _ us)) (snd (hlist_split tus (a0 :: nil) us)) us_).
+              intro XXX; change_rewrite XXX; clear XXX.
+              rewrite hlist_app_hlist_split.
+              generalize (hlist_app us us_).
+              clear. intros.
+              generalize (app_ass_trans tus (a0 :: nil) tus_).
+              simpl. generalize dependent (tus ++ (a0 :: tus_)).
+              intros; subst. reflexivity. }
+            { revert Hfor.
+              clear.
+              generalize (snd (hlist_split tus (a0 :: nil) us)).
+              intro h. rewrite (hlist_eta h).
+              rewrite (hlist_eta (hlist_tl h)).
+              simpl. tauto. }
+            { destruct H2 as [ ? [ ? ? ] ].
+              { revert H2. clear.
+                simpl.
+                rewrite (hlist_eta (snd _)).
+                apply impl_eq. f_equal.
+                rewrite <- hlist_app_nil_r.
+                rewrite hlist_split_hlist_app. reflexivity. } } }
+          { destruct H8 as [ H8 ? ].
+            eapply mapD_nil_conv
+              with (pf__us:=eq_refl) (pf__us':=eq_refl) (pf_vs:=eq_refl)
+                   (pf_us:=app_ass_trans _ _ _)
+                   (pf_us':=eq_refl)
+              in H8.
+            { eexists; split; eauto.
+              intros.
+              inv_all. subst.
+              inst_hlists. clear IHtus_ H8.
+              pose (y1 (hlist_app (hlist_app _us' us') us_') vs : typD a0).
+              simpl in *.
+              destruct (H9 (hlist_app us (Hcons t0 Hnil)) us' us_');
+                clear H9; try eassumption.
+              { autorewrite with eq_rw. eapply H6; clear H6.
+                repeat rewrite hlist_split_hlist_app. simpl.
+                rewrite <- hlist_app_nil_r.
+                rewrite hlist_split_hlist_app. simpl.
+                auto. }
+              { destruct H1.
+                specialize (HeD'eq (Hcons t0 x1) _ HP H1 H10).
+                exists (Hcons t0 x1).
+                rewrite H3; clear H3.
+                rewrite H4; clear H4.
+                simpl.
+                revert HeD'eq. revert H5.
+                autorewrite with eq_rw.
+                rewrite hlist_app_assoc. simpl.
+                generalize (app_ass_trans tus (a0 :: nil) tus_).
+                generalize (hlist_app us (Hcons t0 x1)).
+                simpl.
+                generalize dependent ((tus ++ a0 :: nil) ++ tus_).
+                intros; subst; simpl in *. subst t0.
+                intuition.
+                rewrite HeD'eq. clear.
+                f_equal.
+                rewrite hlist_app_assoc. reflexivity. } }
+            { rewrite app_ass. reflexivity. } } }
+        { (** this is the None case **)
+          specialize (IHtus_ (tus ++ a0 :: nil) (tus' ++ a0::nil) (mlist1_inst ++ None :: nil)).
+          assert (length (_tus ++ tus ++ a0::nil) = S (length (_tus ++ tus))).
+          { repeat rewrite app_length. simpl. omega. }
+          destruct H0.
+          edestruct (fun R pf => @mapD_app_lem _ _ _ _ _ _ _ _ HmapD (a0::nil) (a0::nil) (None::nil)
+                                    (types_after_instantiate tus_
+                                                             (amap_aslist a (length (_tus ++ tus ++ a0::nil)) (length tus_))) R pf eq_refl).
+          { constructor. constructor. }
+          destruct H0.
+          edestruct IHtus_ with (P:=P).
+          { do 2 rewrite app_length. simpl. f_equal. assumption. }
+          { eapply H0. }
+          { revert HsubstD.
+            instantiate (1 := match eq_sym (f_equal (app _tus) (app_ass_trans _ (a0::nil) _)) in _ = t return exprT t _ _ with
+                              | eq_refl => sD'
+                              end).
+            clear.
+            generalize (app_ass_trans tus (a0 :: nil) tus_).
+            generalize ((tus ++ a0 :: nil) ++ tus_). intros; subst.
+            assumption. }
+          { rename H1 into HxR.
+            clear - Hf HxR. intros.
+            destruct (Hf (S n) _ t
+                         match f_equal _ (app_ass_trans _ _ _) in _ = t return exprT t _ _ with
+                         | eq_refl => eD
+                         end H); clear Hf; eauto.
+            { generalize dependent (app_ass_trans tus (a0 :: nil) tus_).
+              generalize dependent ((tus ++ a0 :: nil) ++ tus_).
+              intros; subst. eassumption. }
+            { clear - H1 HxR.
+              exists (match eq_sym (f_equal (app _tus') (app_ass_trans tus' (a0::nil) _)) in _ = t
+                            return exprT t _ _
+                      with
+                      | eq_refl => x0
+                      end).
+              destruct H1.
+              split.
+              { clear - H. revert H.
+                uip_all'. destruct e0. assumption. }
+              { intros. eapply HxR in H1. revert H1. revert HP.
+                clear - H0 Hfor.
+                intros.
+                specialize (H0 _us _us' vs (fst (hlist_split _ _ us))
+                               (fst (hlist_split _ _ us'))
+                               (hlist_app (snd (hlist_split _ _ us)) us_)
+                               (hlist_app (snd (hlist_split _ _ us')) us_')).
+                revert H0.
+                autorewrite with eq_rw.
+                intros.
+                forward_reason.
+                revert H0.
+                clear - HP Hfor H2 H1 H.
+                generalize (hlist_app_assoc' (fst (hlist_split tus (a0::nil) us)) (snd (hlist_split tus (a0::nil) us)) us_).
+                intro XXX. change_rewrite XXX; clear XXX.
+                generalize (hlist_app_assoc' (fst (hlist_split tus' (a0::nil) us')) (snd (hlist_split tus' (a0::nil) us')) us_').
+                intro XXX. change_rewrite XXX; clear XXX.
+                repeat rewrite hlist_app_hlist_split.
+                generalize (app_ass_trans tus' (a0 :: nil)
+                                          (types_after_instantiate tus_
+                                                                   (amap_aslist a (length (_tus ++ tus ++ a0 :: nil))
+                                                                                (length tus_)))).
+                simpl.
+                match goal with
+                | |- forall x : _ = ?X, _ => generalize dependent X; intros; subst
+                end.
+                simpl in *.
+                etransitivity; [ | eapply H0; eauto ].
+                { f_equal.
+                  clear.
+                  generalize (hlist_app us us_).
+                  generalize (app_ass_trans tus (a0 :: nil) tus_).
+                  match goal with
+                  | |- forall x : ?X = _, _ => generalize dependent X; intros; subst
+                  end.
+                  reflexivity. }
+                { clear H0.
+                  generalize dependent (snd (hlist_split tus (a0 :: nil) us)).
+                  generalize dependent (snd (hlist_split _ (a0 :: nil) us')).
+                  clear - Hfor.
+                  intros.
+                  rewrite (hlist_eta h0). rewrite (hlist_eta h).
+                  rewrite (hlist_eta (hlist_tl h0)).
+                  rewrite (hlist_eta (hlist_tl h)).
+                  simpl. split; auto. } } } }
+          { rename H1 into HxR. clear - H2 HxR.
+            exists (match app_ass_trans tus (a0 ::nil) tus_ in _ = t
+                        , app_ass_trans tus' (a0::nil) _ in _ = t'
+                          return _ -> _ -> _ -> hlist _ t -> hlist _ t' -> _ with
+                    | eq_refl , eq_refl => x0
+                    end).
+            destruct H2; split.
+            { clear - H. uip_all'.
+              repeat match goal with
+                     | H : _ = ?X |- _ => generalize dependent X; intros; subst
+                     | H : ?X = _ |- _ => generalize dependent X; intros; subst
+                     end.
+              revert H.
+              rewrite app_ass. auto. }
+            { clear - H0 HxR.
+              intros.
+              generalize (H0 _us _us' vs
+                             (hlist_app us (fst (hlist_split (a0::nil) _ us_')))
+                             (hlist_app us' (fst (hlist_split (a0::nil) _ us_')))
+                             (snd (hlist_split (a0::nil) _ us_'))); clear H0.
+              repeat rewrite hlist_split_hlist_app; simpl.
+              rewrite (hlist_eta us_') in H.
+              destruct 1; eauto.
+              { eapply HxR.
+                repeat rewrite hlist_split_hlist_app; simpl. tauto. }
+              exists (Hcons (hlist_hd us_') x1).
+              revert H0.
+              repeat rewrite hlist_app_assoc. simpl.
+              generalize dependent (app_ass_trans tus (a0 :: nil) tus_).
+              generalize dependent (app_ass_trans tus' (a0 :: nil)
+                                                  (types_after_instantiate tus_
+                                                     (amap_aslist a (length (_tus ++ tus ++ a0 :: nil))
+                                                                  (length tus_)))).
+              intros.
+              repeat match goal with
+                     | H : ?X = _ |- _ => generalize dependent X; intros; subst
+                     end.
+              simpl in *.
+              split; try tauto. rewrite (hlist_eta us_'). simpl. tauto. } } } }
+    Qed.
+
+    Lemma the_actual_lemma'
+    : forall f (_tus _tus' tvs : tenv typ) (a : amap expr)
+        (WFa : FMapSubst.SUBST.WellFormed a),
+        forall (tus_ tus tus' : tenv typ) mlist1_inst mlist2 mlist2_inst
+          (Hlen : length mlist1_inst = length tus),
+          mlist2 = amap_aslist a (length (_tus ++ tus)) (length tus_) ->
+          mlist2_inst = map (Functor.fmap f) mlist2 ->
+          forall R sD' P
+            (HmapD : @mapD _tus
+                  _tus'
+                  (types_after_instantiate tus_ mlist2)
+                  tvs
+                  tus
+                  tus'
+                  mlist1_inst R)
+            (HsubstD : FMapSubst.SUBST.list_substD
+              (_tus ++ tus ++ tus_)
+              tvs
+              (length (_tus ++ tus))
+              mlist2 = Some sD')
+            (Hf : forall (n : nat) e t eD,
+                nth_error mlist2 n = Some (Some e) ->
+                exprD' (_tus ++ tus ++ tus_) tvs e t = Some eD ->
+                exists eD',
+                  exprD' (_tus' ++ tus' ++
+                          types_after_instantiate tus_ mlist2)
+                         tvs (f e) t = Some eD' /\
+                  forall _us _us' vs us us' us_ us_',
+                    P _us _us' vs ->
+                    Forgetting _ us_ us_' ->
+                    R _us _us' vs us us' us_' ->
+                    eD (hlist_app _us (hlist_app us us_)) vs =
+                    eD' (hlist_app _us' (hlist_app us' us_')) vs),
+            exists R',
+              @mapD_nil _tus _tus' tvs (tus ++ tus_)
+                        (tus' ++
+                         types_after_instantiate tus_ mlist2)
+                        (mlist1_inst ++ mlist2_inst)  R' /\
+              forall _us _us' vs us us' us_',
+                P _us _us' vs ->
+                R _us _us' vs us us' us_' ->
+                exists us_,
+                  sD' (hlist_app _us (hlist_app us us_)) vs /\
+                  R' _us _us' vs (hlist_app us us_) (hlist_app us' us_').
+    Proof.
+      clear. intros. subst.
+      eapply the_actual_lemma in HsubstD; eauto.
+      forward_reason.
+      eexists; split; eauto.
+      intros. edestruct H0; eauto.
+      forward_reason; eexists; split; eauto.
+    Qed.
+
+(*
+    Lemma the_actual_lemma_nil'
+    : forall f (_tus _tus' tvs : tenv typ) (a : amap expr)
+        (WFa : FMapSubst.SUBST.WellFormed a),
+        forall (tus_ tus tus' : tenv typ) mlist1_inst mlist2 mlist2_inst
+          (Hlen : length mlist1_inst = length tus),
+          mlist2 = amap_aslist a (length (_tus ++ tus)) (length tus_) ->
+          mlist2_inst = map (Functor.fmap f) mlist2 ->
+          forall R sD' P
+            (HmapD : @mapD_nil _tus
+                  _tus'
+                  tvs
+                  tus
+                  tus'
+                  mlist1_inst R)
+            (HsubstD : FMapSubst.SUBST.list_substD
+              (_tus ++ tus ++ tus_)
+              tvs
+              (length (_tus ++ tus))
+              mlist2 = Some sD')
+            (Hf : forall (n : nat) e t eD,
+                nth_error mlist2 n = Some (Some e) ->
+                exprD' (_tus ++ tus ++ tus_) tvs e t = Some eD ->
+                exists eD',
+                  exprD' (_tus' ++ tus' ++
+                          types_after_instantiate tus_ mlist2)
+                         tvs (f e) t = Some eD' /\
+                  forall _us _us' vs us us' us_ us_',
+                    P _us _us' vs ->
+                    R _us _us' vs us us' ->
+                    eD (hlist_app _us (hlist_app us us_)) vs =
+                    eD' (hlist_app _us' (hlist_app us' us_')) vs),
+            exists R',
+              @mapD_nil _tus _tus' tvs (tus ++ tus_)
+                        (tus' ++
+                         types_after_instantiate tus_ mlist2)
+                        (mlist1_inst ++ mlist2_inst)  R' /\
+              forall _us _us' vs us us' us_',
+                P _us _us' vs ->
+                R _us _us' vs us us' ->
+                exists us_,
+                  sD' (hlist_app _us (hlist_app us us_)) vs /\
+                  R' _us _us' vs (hlist_app us us_) (hlist_app us' us_').
+    Proof.
+      clear. intros.
+      eapply mapD_nil_mapD_iff in HmapD.
+      forward_reason.
+      eapply mapD_weaken_post with (_tus_post':=types_after_instantiate tus_ mlist2) in H1.
+      forward_reason.
+      simpl in *. subst.
+      eapply the_actual_lemma with (f:=f) (P:=P) in H1; eauto.
+      { forward_reason.
+        eexists; split; eauto.
+        intuition. eapply H0; eauto.
+        eapply H2 in H1. eapply H3 in H1. eassumption. }
+      { intros. eapply Hf in H0; eauto.
+        forward_reason; eexists; split; eauto.
+        intros. eapply H4; eauto.
+        eapply H2. eapply H3. simpl. eassumption. }
+    Qed.
+*)
+
+    Lemma do_instantiate_app
+      : forall c (cs : ctx_subst c) base es es' u,
+        do_instantiate cs base (es ++ es') u =
+        if u ?[ lt ] (base + length es) then
+          do_instantiate cs base es u
+        else
+          Some (lookup_compress es' (base + length (filter (fun x => match x with
+                                                                     | Some _ => false
+                                                                     | None => true
+                                                                     end) es))
+                                (u - base - length es)).
+    Proof.
+      clear. intros.
+      unfold do_instantiate.
+      generalize (lt_rem_sound base u).
+      destruct (lt_rem u base); intros.
+      { destruct H. subst.
+        consider (u ?[ lt ] (base + length es)).
+        { intros. rewrite lookup_compress_app.
+          consider ((u - base) ?[ lt ] length es); auto.
+          intros. exfalso. omega. }
+        { intros. rewrite lookup_compress_app.
+          consider ((u - base) ?[ lt ] length es); auto.
+          { intros. exfalso. omega. } } }
+      { consider (u ?[ lt ] (base + length es)); auto.
+        intros.
+        exfalso; omega. }
+    Qed.
+
+    Lemma mapD_nil_weaken_tvs
+    : forall _tus _tus' _tvs _tvs' tus tus' es P,
+        @mapD_nil _tus _tus' _tvs tus tus' es P ->
+        exists P',
+          @mapD_nil _tus _tus' (_tvs ++ _tvs') tus tus' es P' /\
+          forall U U' V V' a b,
+            P U U' V a b <-> P' U U' (hlist_app V V') a b.
+    Proof.
+      induction 1; simpl; intros.
+      { eexists. split. constructor.
+        simpl. intros; tauto. }
+      { forward_reason.
+        eexists; split.
+        - econstructor. eauto.
+        - simpl. intros. rewrite H1. reflexivity. }
+      { eapply exprD'_weakenV with (tvs':=_tvs') in H0; eauto.
+        forward_reason.
+        eexists; split.
+        - econstructor; eauto.
+        - simpl. intros.
+          rewrite <- H2. rewrite <- H3. reflexivity. }
+    Qed.
+
+    Lemma minify_goal_sound_lem
     : forall g tus tvs tus' es g',
         minify_goal es (length (getUVars c ++ tus)) g = g' ->
-        WellFormed_Goal (getUVars c ++ tus) tvs g ->
-        WellFormed_Goal (getUVars c ++ tus') tvs g' /\
-        forall gD sD R,
-          goalD (getUVars c ++ tus) tvs g = Some gD ->
-          substD (getUVars c) tvs cs = Some sD ->
-          @mapD (getUVars c) (getUVars c) tvs tus tus' es R ->
+        WellFormed_Goal (getUVars c ++ tus) (getVars c ++ tvs) g ->
+        WellFormed_Goal (getUVars c ++ tus') (getVars c ++ tvs) g' /\
+        forall gD (sD : exprT (getUVars c) (getVars c) Prop) R,
+          goalD (getUVars c ++ tus) (getVars c ++ tvs) g = Some gD ->
+          forall (Hsubst : substD (getUVars c) (getVars c) cs = Some sD)
+                 (Hes_tus_len : length es = length tus),
+          @mapD_nil (getUVars c) (getUVars c) (getVars c ++ tvs) tus tus' es R ->
           exists gD',
-            goalD (getUVars c ++ tus') tvs g' = Some gD' /\
-            forall _us _vs us us',
-              R _us _us _vs us us' ->
+            goalD (getUVars c ++ tus') (getVars c ++ tvs) g' = Some gD' /\
+            forall _us _vs vs us us',
+              R _us _us (hlist_app _vs vs) us us' ->
               sD _us _vs ->
-              (gD' (hlist_app _us us') _vs <->
-               gD (hlist_app _us us) _vs).
+              (gD' (hlist_app _us us') (hlist_app _vs vs) ->
+               gD (hlist_app _us us) (hlist_app _vs vs)).
     Proof.
       induction g.
       { (* All *)
-(*
+        clear base_is_nus.
         simpl. intros. inv_all.
-        specialize (@IHg tus (tvs ++ t :: nil) tus' es _ _ eq_refl H0
-                         (@mapD_weaken_tvs _ _ (t :: nil) _ _ _ _ H1));
-          forward_reason.
-        destruct (@GAll_do_solved_respects _ _ _ _ _ (getUVars c ++ tus') tvs t
-                   _ _ (Reflexive_EqGoal _ _ (minify_goal es (length (getUVars c ++ tus)) g))). *)
-(*
+        specialize (IHg tus (tvs ++ t :: nil) tus' es _ eq_refl).
+        destruct IHg.
+        { rewrite app_ass in H0. assumption. }
         split.
-        { subst. eapply H4.
-          constructor; assumption. }
+        { subst. eapply WellFormed_Goal_GAll_do_solved. constructor.
+          rewrite app_ass. assumption. }
         intros; forward; inv_all; subst.
         simpl.
-        specialize (H6 _ eq_refl).
-        forward_reason; Cases.rewrite_all_goal.
-        simpl in H5. rewrite H in H5.
-        inversion H5.
+        generalize (@GAll_do_solved_respects typ expr _ _ _ (getUVars c ++ tus')
+                                             (getVars c ++ tvs) t
+                    _ _ (Reflexive_EqGoal _ _ (minify_goal es (length (getUVars c ++ tus)) g))).
+        destruct 1. clear H.
+        rewrite goalD_conv
+           with (pfu:=eq_refl) (pfv:=eq_sym (app_ass_trans _ _ _)) in H3.
+        autorewrite with eq_rw in H3. forwardy. inv_all; subst.
+        destruct (mapD_nil_weaken_tvs (t::nil) H4) as [ ? [ ? ? ] ].
+        eapply mapD_nil_conv
+          with (pf_us':=eq_refl) (pf_us:=eq_refl) (pf_vs:=app_ass_trans _ _ _)
+               (pf__us:=eq_refl) (pf__us':=eq_refl)
+          in H3; [ | reflexivity ].
+        specialize (H2 _ _ _ H Hsubst Hes_tus_len H3).
+        forward_reason.
+        rewrite goalD_conv
+           with (pfu:=eq_refl) (pfv:=app_ass_trans _ _ _) in H2.
+        autorewrite with eq_rw in H2. forwardy.
+        simpl in H5. change_rewrite H2 in H5.
+        inversion H5; clear H5; subst.
         eexists; split; eauto.
-        simpl. intros. subst.
-        etransitivity. eapply H9. reflexivity. reflexivity.
-        eapply forall_iff. intro.
-        specialize (H6 _us (hlist_app _vs (Hcons x1 Hnil)) us us').
-        rewrite hlist_split_hlist_app in H6. simpl in H6. eauto. *) admit. }
+        inv_all; subst.
+        intros.
+        autorewrite with eq_rw.
+        generalize (H7 _us _vs (hlist_app vs (Hcons x0 Hnil)) us us'); clear H7. intros.
+        rewrite <- hlist_app_assoc'.
+        eapply H7; eauto.
+        { autorewrite with eq_rw.
+          rewrite <- hlist_app_assoc.
+          eapply H6. eassumption. }
+        { autorewrite with eq_rw.
+          rewrite <- hlist_app_assoc.
+          eapply H11 in H10; first [ eassumption | reflexivity ]. } }
+
       { (* Exs *)
         cbv beta iota delta [ minify_goal ]; fold minify_goal.
         intros.
         simpl in H.
         remember (amap_aslist a (length (getUVars c ++ tus)) (length l)) as mlist.
-        remember (combine l
-                   (map
-                      (fun x : option expr =>
-                       match x with
-                       | Some x0 =>
-                           Some
-                             (instantiate (do_instantiate cs base (es ++ mlist))
-                                0 x0)
-                       | None => None
-                       end) mlist)) as tes.
-        remember (map fst
-                    (filter
-                       (fun x : typ * option expr =>
-                          match snd x with
-                            | Some _ => false
-                            | None => true
-                          end) tes)) as ts'.
+        match goal with
+          | _ : GExs_nil_check ?X _ _ = _ |- _ =>
+            remember X as ts'
+        end.
         remember (map
                     (fun x : option expr =>
                        match x with
@@ -640,9 +1727,9 @@ Section parameterized.
                         eq_refl H1).
         forward_reason.
         destruct (@GExs_nil_check_respects _ _ _ _ _ _
-                    (getUVars c ++ tus') tvs ts' (amap_empty expr)
+                    (getUVars c ++ tus') (getVars c ++ tvs) ts' (amap_empty expr)
                     (only_in_range_empty _ _)
-                    (WellFormed_amap_amap_empty) _ _
+                    (@WellFormed_amap_amap_empty _ _ _ _ _) _ _
                     (Reflexive_EqGoal _ _
                        (minify_goal (es ++ mlist_inst)
                           (length ts + length (getUVars c ++ tus)) g))).
@@ -659,55 +1746,365 @@ Section parameterized.
           end.
           f_equal. f_equal. omega. }
         clear H4.
-        rewrite H in *. clear H. (* Can I do this? *)
-        simpl in *; intros. forward; inv_all. subst gD.
-        rewrite goalD_conv with (pfu:=eq_sym (app_ass_trans _ _ _)) (pfv:=eq_refl) in H.
-        autorewrite with eq_rw in H. forward.
-        pose (R':=fun U U' V (a : hlist typD (tus ++ ts))
-                        (b : hlist typD (tus' ++ ts')) =>
-                      R U U' V (fst (hlist_split _ _ a)) (fst (hlist_split _ _ b))
-                      /\ e0 (hlist_app (hlist_app U (fst (hlist_split _ _ a)))
-                                       (snd (hlist_split _ _ a)))  V).
-        assert (exists R'',
-                   mapD (tus ++ ts) (tus' ++ ts') (es ++ mlist_inst) R'' /\
-                   forall _us _us' _vs a b,
-                     R'' _us _us' _vs a b <-> R' _us _us' _vs a b).
-        { clear H3 H H5. revert H6.
-          revert H7. subst mlist_inst.
-          revert Heqmlist. revert H2. subst R'.
-          revert Heqts'. subst tes.
-          clear. revert e0. revert R.
-          revert mlist ts' es. revert tus tvs tus'. revert a.
-          induction ts.
-          { simpl. intros; subst. simpl in *.
-            clear - H6 H7.
-            eapply mapD_conv
-              with (pf_us:=eq_sym (app_nil_r_trans _))
-                   (pf_vs:=eq_sym (app_nil_r_trans _))
-                   (es':=es++nil)
-              in H6; [ | symmetry; eapply app_nil_r_trans ].
+        rewrite H in *; clear  H.
+        simpl in *; intros. forwardy; inv_all. subst gD.
+        rewrite goalD_conv
+           with (pfu:=eq_sym (app_ass_trans _ _ _)) (pfv:=eq_refl)
+             in H.
+        autorewrite with eq_rw in H. forwardy.
+        inv_all. subst y.
+        eapply amap_substD_list_substD in H6; eauto.
+
+        assert (Hmlist_ts_length : length ts = length mlist).
+        { clear - Heqmlist. symmetry. eapply length_list_subst. eauto. }
+        assert (Hes_tus_len' : length (es ++ mlist_inst) = length (tus ++ ts)).
+        { do 2 rewrite app_length. rewrite Hmlist_ts_length.
+          rewrite Hes_tus_len. f_equal.
+          subst mlist_inst. rewrite map_length. reflexivity. }
+        specialize (fun R => H3 _ _ R H Hsubst Hes_tus_len').
+        generalize H4; intro H_remember_mapD_nil.
+
+        change (fun x2 : option expr =>
+                  match x2 with
+                  | Some x3 =>
+                    Some
+                      (instantiate
+                         (do_instantiate cs base (es ++ mlist)) 0
+                         x3)
+                  | None => None
+                  end)
+          with (Functor.fmap (F:=option) (instantiate (do_instantiate cs base (es ++ mlist)) 0)) in *.
+        forward_reason.
+        eapply mapD_nil_mapD_iff in H4.
+        destruct H4 as [ ? [ H4 Heq_mapD_mapD_nil ] ].
+        eapply mapD_weaken_post
+          with (_tus_post':=types_after_instantiate ts mlist)
+            in H4.
+        destruct H4 as [ ? [ H4 Heq_mapD_weaken ] ].
+        rewrite <- Heqmlist in H6.
+        erewrite list_substD_conv
+           with (pfu:=app_ass_trans _ _ _) (pfv:=eq_refl) in H6 by reflexivity.
+        simpl in H6; autorewrite with eq_rw in H6. forwardy.
+        destruct (fun H =>
+                      @the_actual_lemma'
+                        (instantiate (do_instantiate cs base (es ++ mlist)) 0)
+                        (getUVars c) (getUVars c) (getVars c ++ tvs) a H
+                        ts tus tus' es mlist mlist_inst Hes_tus_len Heqmlist Heqmlist_inst
+                        _ _ (fun us us' vs => us = us' /\ sD us' (fst (hlist_split _ _ vs))) H4 H6).
+        { destruct H2. tauto. }
+        { (** Side condition **)
+          revert H4. revert H6. revert Heqmlist Heqmlist_inst. revert H2.
+          clear - Hes_tus_len Hmlist_ts_length base_is_nus RTypeOk_typ ExprOk_expr
+                  ExprUVarOk_expr H_remember_mapD_nil Hsubst
+                  Heq_mapD_weaken Heq_mapD_mapD_nil.
+          simpl; intros H2 Heqmlist Heqmlist_inst H6 H4 n e t eD H H0.
+          unfold instantiate in *.
+          edestruct (@expr_subst_sound _ _ _ _ _
+                         (do_instantiate cs base (es ++ mlist)) (fun _ => None)
+                         0 e _ eq_refl nil
+                         (getUVars c ++ tus ++ ts) (getVars c ++ tvs)
+                         (getUVars c ++ tus' ++ types_after_instantiate ts mlist) (getVars c ++ tvs)
+          (fun us vs us' vs' =>
+             vs = vs' /\
+             sD (fst (hlist_split _ _ us')) (fst (hlist_split _ _ vs)) /\
+             fst (hlist_split _ _ us) = fst (hlist_split _ _ us') /\
+             x1 (fst (hlist_split _ _ us)) (fst (hlist_split _ _ us')) vs
+                (fst (hlist_split _ _ (snd (hlist_split _ _ us))))
+                (fst (hlist_split _ _ (snd (hlist_split _ _ us'))))
+                (snd (hlist_split _ _ (snd (hlist_split _ _ us')))) /\
+             Forgetting mlist
+                        (snd (hlist_split _ _ (snd (hlist_split _ _ us))))
+                        (snd (hlist_split _ _ (snd (hlist_split _ _ us'))))));
+            try first [ reflexivity | eassumption ].
+          { clear H0 eD.
+            intros.
+            assert (u < length (getUVars c ++ tus) \/
+                    (u >= length (getUVars c ++ tus) /\
+                     nth_error mlist (u - length (getUVars c ++ tus)) = Some None)).
+            { assert (u < length (getUVars c ++ tus) \/ u >= length (getUVars c ++ tus)) by omega.
+              destruct H3; auto.
+              right. split; auto.
+              apply nth_error_get_hlist_nth_Some in H1.
+              simpl in H1. forward_reason.
+              clear H1.
+              apply ListNth.nth_error_length_lt in x.
+              clear - H0 H3 H H6 Heqmlist H2 x.
+              subst. rewrite amap_aslist_nth_error.
+              rewrite rel_dec_eq_true; eauto with typeclass_instances.
+              { rewrite amap_aslist_nth_error in H.
+                consider (n ?[ lt ] length ts); try congruence. intros.
+                inv_all. destruct H2.
+                eapply H2 in H1. red in H1.
+                eapply H1 in H0.
+                cutrewrite (length (getUVars c ++ tus) + (u - length (getUVars c ++ tus)) = u); [ | omega ].
+                f_equal.
+                unfold amap_lookup.
+                apply FMapSubst.SUBST.FACTS.not_find_in_iff. assumption. }
+              { clear - x H3.
+                repeat rewrite app_length in *. omega. } }
+            clear H0.
+            rewrite do_instantiate_app.
+            destruct H3.
+            { rewrite rel_dec_eq_true.
+              2: eauto with typeclass_instances.
+              Focus 2. rewrite Hes_tus_len. subst base. rewrite <- app_length. assumption.
+              rewrite nth_error_get_hlist_nth_conv with (pf:=app_ass_trans _ _ _) in H1.
+              autorewrite with eq_rw in H1.
+              forwardy.
+              eapply nth_error_get_hlist_nth_appL in H0.
+              setoid_rewrite H1 in H0.
+              forward_reason.
+              eapply do_instantiate_sound with (es:=es) (tus':=tus') (tvs:=tvs) in H5; eauto.
+              { destruct (do_instantiate cs base es u).
+                { forward_reason.
+                  eapply exprD'_weakenU with (tus':=types_after_instantiate ts mlist) in H5;
+                    eauto with typeclass_instances.
+                  forward_reason.
+                  rewrite exprD'_conv
+                     with (pfu:=eq_sym (app_ass_trans _ _ _)) (pfv:=eq_refl) in H5.
+                  autorewrite with eq_rw in H5. forwardy.
+                  inv_all. subst. subst.
+                  autorewrite with eq_rw in H3.
+                  inv_all. subst.
+                  eexists; split; try eassumption.
+                  subst. intros us vs us' vs'.
+                  simpl; intros; forward_reason.
+                  subst.
+                  simpl in *.
+                  Ltac shatter hl :=
+                    let rec it hl k :=
+                        match type of hl with
+                        | hlist ?T (?X ++ ?Y) =>
+                          it (fst (hlist_split _ _ hl)) ltac:(fun x =>
+                            it (snd (hlist_split _ _ hl)) ltac:(fun y =>
+                              k (hlist_app x y)))
+                        | _ => k hl
+                        end
+                    in
+                    let rec f hl :=
+                        match type of hl with
+                        | hlist ?T (?X ++ ?Y) =>
+                          f (fst (hlist_split _ _ hl)) ;
+                          f (snd (hlist_split _ _ hl))
+                        | _ => generalize dependent hl
+                        end
+                    in
+                    it hl ltac:(fun x => assert (hl = x) by
+                                          (repeat (rewrite hlist_app_hlist_split; simpl) ; reflexivity) ; f hl ; intros).
+                  shatter us; shatter us'; shatter vs'.
+                  specialize (H9 (hlist_app h4 h3) (hlist_app h6 h5) h2).
+                  specialize (H8 (hlist_app h1 h0) h6 h5 (hlist_app h4 h3) h5).
+                  specialize (H7 (hlist_app h1 h0) h).
+                  revert H9.
+                  autorewrite with eq_rw.
+                  rewrite <- hlist_app_assoc'.
+                  subst. rewrite <- hlist_app_assoc.
+                  repeat rewrite hlist_split_hlist_app in H8. simpl in H8.
+                  intros. etransitivity; eauto.
+                  etransitivity; [ eapply H8; auto | eauto ].
+                  split; auto. split; auto.
+                  eapply Heq_mapD_mapD_nil; clear Heq_mapD_mapD_nil.
+                  eapply Heq_mapD_weaken; eauto. }
+                { forward_reason.
+                  eapply nth_error_get_hlist_nth_weaken
+                    with (ls':=types_after_instantiate ts mlist)
+                      in H5.
+                  simpl in H5; forward_reason.
+                  rewrite nth_error_get_hlist_nth_conv
+                     with (pf:=eq_sym (app_ass_trans _ _ _)) in H5.
+                  autorewrite with eq_rw in H5.
+                  forwardy.
+                  inv_all; subst.
+                  destruct y1.
+                  autorewrite with eq_rw in H3.
+                  inv_all; subst. subst.
+                  autorewrite with eq_rw in H10.
+                  inv_all; subst; subst. simpl in *. subst.
+                  eexists; split; eauto.
+                  subst. intros; forward_reason.
+                  subst.
+                  shatter us; shatter us'.
+                  specialize (H9 (hlist_app h4 h3) h2).
+                  specialize (H7 (hlist_app h1 h0) h).
+                  specialize (H8 (hlist_app h1 h0)).
+                  revert H9.
+                  autorewrite with eq_rw.
+                  rewrite <- hlist_app_assoc'.
+                  subst. rewrite <- hlist_app_assoc.
+                  intros. etransitivity; eauto.
+                  etransitivity; [ | eassumption ].
+                  eapply H8; clear H8.
+                  repeat rewrite hlist_split_hlist_app. simpl.
+                  split; [ | split; [ | split ] ].
+                  reflexivity. 3: eassumption.
+                  reflexivity.
+                  eapply Heq_mapD_mapD_nil.
+                  eapply Heq_mapD_weaken.
+                  simpl.
+                  instantiate (2:=
+                                 snd (hlist_split (getVars c) tvs vs')).
+                  rewrite hlist_app_hlist_split.
+                  eassumption. } } }
+
+            { rewrite rel_dec_neq_false.
+              2: eauto with typeclass_instances.
+              Focus 2. rewrite Hes_tus_len. subst base. rewrite <- app_length. omega.
+              subst base. rewrite Hes_tus_len.
+              assert (length
+                        (filter
+                           (fun x : option expr =>
+                              match x with
+                              | Some _ => false
+                              | None => true
+                              end) es) = length tus').
+              { clear - H4.
+                induction H4; (** lemma **)
+                  solve [ reflexivity | simpl; assumption | simpl; f_equal; assumption ]. }
+              rewrite H3.
+              rewrite <- app_length.
+              eapply nth_error_get_hlist_nth_appR in H1; simpl in H1; forward_reason.
+              eapply nth_error_get_hlist_nth_appR in H1; simpl in H1; forward_reason.
+              replace (u - length (getUVars c) - length tus)
+                 with (u - length (getUVars c ++ tus))
+                   in *
+                   by (rewrite app_length; clear; omega).
+              Focus 2. rewrite app_length in H0. omega.
+              Focus 2. rewrite app_length in H0. omega.
+              clear H.
+              generalize dependent (u - length (getUVars c ++ tus)).
+              clear H0. clear u.
+              clear Heqmlist_inst mlist_inst H3.
+              assert (forall u,
+                      nth_error_get_hlist_nth typD ts u =
+                      Some (existT (fun t1 : typ => hlist typD ts -> typD t1) t0 x2) ->
+                      nth_error mlist u = Some None ->
+                      exists
+                        eUD : exprT (getUVars c ++ tus' ++ types_after_instantiate ts mlist)
+                                    (getVars c ++ tvs) (typD t0),
+                        exprD' (getUVars c ++ tus' ++ types_after_instantiate ts mlist)
+                               (getVars c ++ tvs)
+                               (lookup_compress mlist (length (getUVars c ++ tus')) u) t0 = 
+                        Some eUD /\
+                        (forall (usa : hlist typD (getUVars c ++ tus))
+                                (usc : hlist typD ts)
+                                (usa' : hlist typD (getUVars c ++ tus'))
+                                (usc' : hlist typD (types_after_instantiate ts mlist))
+                                (vs' : hlist typD (getVars c ++ tvs)),
+                            Forgetting mlist usc usc' ->
+                            x2 usc = eUD match app_ass_trans _ _ _ in _ = t return hlist _ t with
+                                         | eq_refl => hlist_app usa' usc'
+                                         end vs')).
+              { clear - ExprUVarOk_expr RTypeOk_typ.
+                intro u.
+                destruct (app_ass_trans (getUVars c) tus' (types_after_instantiate ts mlist)).
+                generalize dependent (getUVars c ++ tus').
+                revert mlist; revert x2; revert ts.
+                induction u; simpl; intros.
+                { destruct mlist; simpl in *.
+                  - inversion H0.
+                  - inversion H0; clear H0; subst.
+                    destruct ts; simpl in *; try congruence.
+                    inv_all; subst. subst.
+                    destruct (exprD'_exact_uvar l (types_after_instantiate ts mlist) (getVars c ++ tvs) t).
+                    forward_reason.
+                    eexists; split; eauto.
+                    intros.
+                    rewrite (hlist_eta usc').
+                    rewrite H0. tauto. }
+                { destruct mlist; simpl in *.
+                  - inversion H0.
+                  - destruct ts. simpl in *. try congruence.
+                    simpl in H. forwardy. inv_all. subst. subst.
+                    destruct o; simpl.
+                    { specialize (IHu ts t1 mlist l H H0).
+                      forward_reason. eauto. }
+                    { specialize (IHu ts t1 mlist (l++t::nil) H H0).
+                      forward_reason.
+                      rewrite exprD'_conv with (pfv:=eq_refl)(pfu:=eq_sym (app_ass_trans _ _ _)) in H1.
+                      autorewrite with eq_rw in H1. forwardy.
+                      inv_all; subst.
+                      rewrite app_length in H1. simpl in H1.
+                      rewrite Plus.plus_comm in H1.
+                      eexists; split; eauto.
+                      intros. destruct H3.
+                      erewrite (H2 usa (hlist_tl usc) (hlist_app usa' (Hcons (hlist_hd usc') Hnil)) _ vs') by eauto.
+                      clear.
+                      autorewrite with eq_rw.
+                      f_equal. rewrite hlist_app_assoc.
+                      autorewrite with eq_rw. simpl. rewrite (hlist_eta usc').
+                      reflexivity. } } }
+              { clear - H H8 H7.
+                intros. eapply H in H1; eauto.
+                forward_reason.
+                eexists; split; eauto.
+                intros.
+                rewrite <- (hlist_app_hlist_split _ _ us).
+                rewrite H7; clear H7.
+                rewrite <- (hlist_app_hlist_split _ _ (snd (hlist_split _ _ us))).
+                rewrite H8; clear H8.
+                specialize (H1 (hlist_app (fst (hlist_split _ _ us))
+                                          (fst (hlist_split _ _ (snd (hlist_split _ _ us)))))
+                               (snd (hlist_split _ _ (snd (hlist_split _ _ us))))
+                               (hlist_app (fst (hlist_split _ _ us'))
+                                          (fst (hlist_split _ _ (snd (hlist_split _ _ us')))))
+                               (snd (hlist_split _ _ (snd (hlist_split _ _ us')))) vs').
+                forward_reason. rewrite H1.
+                clear. rewrite <- hlist_app_assoc'.
+                rewrite hlist_app_hlist_split; simpl.
+                rewrite hlist_app_hlist_split; simpl. reflexivity. } } }
+          { intros. rewrite H3. eexists; split; eauto.
+            clear. intros; intuition. subst. reflexivity. }
+          { destruct H1.
             eexists; split; eauto.
             intros.
-            autorewrite with eq_rw.
-            rewrite (hlist_eta (snd (hlist_split _ _ a0))).
-            rewrite hlist_app_nil_r.
-            admit. }
-          { admit. } }
-(*
-        specialize (H3 _ _ R' eq_refl H4 H9).
-        forward_reason.
-        revert H5.
-        rewrite goalD_conv with (pfu:=eq_sym (app_ass_trans _ _ _)) (pfv:=eq_refl). autorewrite with eq_rw.
-        revert H3. repeat rewrite app_length.
-        replace (length (getUVars c) + (length tus + length ts))
-           with (length ts + (length (getUVars c) + length tus)) by omega.
-        intro XXX; rewrite XXX.
-        inversion 1. eexists; split; eauto.
-        intros. do 5 red in H12.
-        etransitivity; [ symmetry; eapply H12; reflexivity | ].
-*)
-        (** TODO(gmalecha): this should work out **)
-        admit. (* hard *) }
+            specialize (H3 (hlist_app _us (hlist_app us us_))
+                           vs
+                           (hlist_app _us' (hlist_app us' us_'))
+                           vs Hnil).
+            simpl in *.
+            eapply H3; clear H3.
+            repeat (rewrite hlist_split_hlist_app; simpl).
+            tauto. } }
+        { destruct H9. subst ts'.
+          assert (Heq_types_after :
+                    types_after_instantiate ts mlist = types_after_instantiate ts mlist_inst).
+          { subst mlist_inst.
+            symmetry. eapply types_after_instantiate_map_fmap. }
+          destruct Heq_types_after.
+          destruct (H3 _ H9) as [ ? [ HgoalD Hres ] ]; clear H3.
+          rewrite goalD_conv
+             with (pfu:=app_ass_trans _ _ _)
+                  (pfv:=eq_refl) in HgoalD.
+          autorewrite with eq_rw in HgoalD.
+          replace (length (getUVars c ++ tus ++ ts))
+             with (length ts + length (getUVars c ++ tus))
+               in HgoalD by (repeat rewrite app_length; omega).
+          forwardy.
+          rewrite H3 in H5; clear H3.
+          inversion H5; clear H5.
+          eexists; split; eauto.
+          subst x4. clear H12.
+          intros.
+          eapply H13 in H12; try reflexivity.
+          apply Quant._exists_sem in H12.
+          destruct H12.
+          destruct (H10 _us _us (hlist_app _vs vs) us us' x4); clear H10.
+          { rewrite hlist_split_hlist_app. split; eauto. }
+          { eapply (fun U U' => Heq_mapD_weaken U U' Hnil).
+            eapply Heq_mapD_mapD_nil; eauto. }
+          apply Quant._exists_sem.
+          exists x5.
+          rewrite H7; clear H7.
+          inv_all. subst.
+          autorewrite with eq_rw.
+          do 2 rewrite <- hlist_app_assoc'.
+          clear H0 H9.
+          destruct H14; split; auto.
+          eapply Hres; eauto.
+          autorewrite with eq_rw.
+          rewrite <- hlist_app_assoc.
+          tauto. } }
+
       { (* Hyp *)
         simpl. intros.
         inv_all.
@@ -718,27 +2115,26 @@ Section parameterized.
           constructor. eauto. }
         { intros.
           forwardy. inv_all; subst.
-          eapply instantiate_do_instantiate_sound in H3; eauto.
+          eapply instantiate_do_instantiate_propD_sound in H3; eauto.
           forward_reason.
           generalize (@GHyp_do_solved_respects typ expr _ _ _ _ _ _ _ H).
           unfold EqGoal; simpl. intros.
-          red in H7.
-          destruct (H7 (minify_goal es (length (getUVars c ++ tus)) g) (minify_goal es (length (getUVars c ++ tus)) g)); clear H7.
+          red in H6.
+          destruct (H6 (minify_goal es (length (getUVars c ++ tus)) g) (minify_goal es (length (getUVars c ++ tus)) g)); clear H6.
           { clear. split; eauto. reflexivity.
             apply Option.Reflexive_Roption.
             eapply Reflexive_RexprT. eauto with typeclass_instances. }
-          revert H9; simpl.
-          eapply H2 in H6; clear H2; eauto.
+          revert H8; simpl.
+          eapply H2 in H5; clear H2; eauto.
           forward_reason.
           Cases.rewrite_all_goal.
-          intros. inversion H9; clear H9; subst.
+          intros. inversion H8; clear H8; subst.
           eexists; split; eauto.
           intros.
-          specialize (H6 _ _ _ _ H9 H10).
-          specialize (H3 _ _ _ _ H9 H10).
-          rewrite <- H6; clear H6.
-          rewrite <- H3; clear H3.
-          eapply H11. reflexivity. reflexivity. } }
+          eapply (H5 _us _vs vs us us'); clear H5; eauto.
+          eapply H10; try reflexivity. eauto.
+          eapply H3; eauto. } }
+
       { (* Conj *)
         simpl. intros.
         inv_all.
@@ -750,11 +2146,11 @@ Section parameterized.
         intros.
         forwardy; inv_all.
         subst gD.
-        specialize (H3 _ _ _ H9 H7 H8).
-        specialize (H5 _ _ _ H6 H7 H8).
+        specialize (H3 _ _ _ H8 Hsubst Hes_tus_len H7).
+        specialize (H5 _ _ _ H6 Hsubst Hes_tus_len H7).
         forward_reason.
         subst g'.
-        destruct (@GConj_GConj_ typ expr _ _ _ _ (getUVars c ++ tus') tvs
+        destruct (@GConj_GConj_ typ expr _ _ _ _ (getUVars c ++ tus') (getVars c ++ tvs)
                                 (minify_goal es (length (getUVars c ++ tus)) g1)
                                 (minify_goal es (length (getUVars c ++ tus)) g1)
                                 (Reflexive_EqGoal _ _ _)
@@ -769,22 +2165,30 @@ Section parameterized.
         subst.
         eexists; split; [ reflexivity | ].
         intros.
-        rewrite <- (H10 _ _ _ _ H14 H16).
-        rewrite <- (H11 _ _ _ _ H14 H16).
-        do 5 red in H15. rewrite H15; [ clear H15 | reflexivity | reflexivity ].
-        reflexivity. }
+        generalize (H9 _us _vs vs us us' H13 H15); clear H9.
+        generalize (H10 _us _vs _ _ _ H13 H15); clear H10.
+        intros.
+        eapply H14 in H16; try reflexivity.
+        split.
+        { eapply H9; eauto. tauto. }
+        { eapply H10; eauto. tauto. } }
+
       { (* Goal *)
         intros. clear base_is_nus. subst.
         split.
         { constructor. }
         simpl in *. intros.
-        eapply instantiate_do_instantiate_sound; eauto. }
+        eapply instantiate_do_instantiate_propD_sound in H; eauto.
+        forward_reason.
+        eexists; split; eauto.
+        intros.
+        eapply H2; eauto. }
+
       { (* Solved *)
         intros; clear base_is_nus; subst.
         split; [ constructor | ].
         intros; inv_all; subst.
-        simpl. eexists; split; eauto.
-        simpl. reflexivity. }
+        simpl. eexists; split; eauto. }
     Qed.
 
   End minify.
@@ -801,47 +2205,35 @@ Section parameterized.
     red.
     intros.
     rewrite <- (app_nil_r_trans (getUVars ctx)) in H.
-    destruct (@minify_goal_sound _ _ s eq_refl H0 g nil
-                                 (getVars ctx) nil nil _ eq_refl H).
+    rewrite <- (app_nil_r_trans (getVars ctx)) in H.
+    destruct (@minify_goal_sound_lem (length (getUVars ctx)) _ s eq_refl H0 g nil nil nil nil _ eq_refl H).
     split; auto.
     split.
-    { clear - H1. rewrite app_nil_r_trans in H1. assumption. }
+    { clear - H1. repeat rewrite app_nil_r_trans in H1. assumption. }
     forward.
     rewrite goalD_conv with (pfu:=app_nil_r_trans _) (pfv:=eq_refl) in H4.
     autorewrite with eq_rw in H4.
     forward.
     destruct (@pctxD_substD  _ _ _ _ _ _ _ _ _ _ H0 H3); forward_reason.
-    specialize (H4 _ _ _ eq_refl H6 (@MD_nil _ _ _ _)).
+    rewrite goalD_conv with (pfv:=app_nil_r_trans _) (pfu:=eq_refl) in H4.
+    autorewrite with eq_rw in H4.
+    forwardy.
+    specialize (H2 _ _ _ H4 H6 eq_refl (@MD_nil_nil _ _ _)).
     forward_reason.
     inv_all; subst.
     rewrite goalD_conv with (pfu:=app_nil_r_trans _) (pfv:=eq_refl).
     autorewrite with eq_rw.
     cutrewrite (minify_goal (length (getUVars ctx)) s nil (length (getUVars ctx)) g = minify_goal (length (getUVars ctx)) s nil (length (getUVars ctx ++ nil)) g).
-    { rewrite H4.
+    { rewrite goalD_conv with (pfu:=eq_refl) (pfv:=app_nil_r_trans _).
+      autorewrite with eq_rw.
+      rewrite H2.
       split; [ reflexivity | ].
       intros. gather_facts.
-      eapply Pure_pctxD; eauto. clear - H8.
-      intros. specialize (H8 us vs Hnil Hnil eq_refl H).
+      eapply Pure_pctxD; eauto. clear - H9.
+      intros. specialize (H9 us vs Hnil Hnil _ eq_refl H).
       revert H0. autorewrite with eq_rw.
-      rewrite <- hlist_app_nil_r. eapply H8. }
+      repeat rewrite <- hlist_app_nil_r. eapply H9. }
     { f_equal. rewrite app_nil_r_trans. reflexivity. }
   Qed.
 
 End parameterized.
-
-(*
-Lemma minify_goal_sound
-    : forall g tus tvs tus' es g' R,
-        (minify_goal es (length (getUVars c ++ tus)) g) = g' ->
-        WellFormed_Goal (getUVars c ++ tus) (getVars c ++ tvs) g ->
-        @mapD (getUVars c) (getVars c ++ tvs) tus tus' es R ->
-        WellFormed_Goal (getUVars c ++ tus') (getVars c ++ tvs) g' /\
-        forall gD,
-          goalD (getUVars c ++ tus) (getVars c ++ tvs) g = Some gD ->
-          exists gD',
-            goalD (getUVars c ++ tus') (getVars c ++ tvs) g' = Some gD' /\
-            forall _us _vs us us' vs,
-              R _us (hlist_app _vs vs) us us' ->
-              (gD' (hlist_app _us us') (hlist_app _vs vs) <->
-               gD (hlist_app _us us) (hlist_app _vs vs)).
-*)
